Work on wordcountProof for ag32

examples/compilation/ag32/proofs/wordcountProofScript.sml
@@ -6,6 +6,16 @@ val _ = new_theory"wordcountProof";
 
 val is_ag32_init_state_def = ag32_targetTheory.is_ag32_init_state_def;
 
+val get_mem_word_get_byte =
+  ag32_basis_ffiTheory.get_mem_word_get_byte
+  |> Q.GEN`r0` |> Q.SPEC`0w` |> SIMP_RULE(srw_ss())[EVAL``byte_aligned 0w``]
+
+val target_state_rel_ag32_init =
+  ag32_basis_ffiTheory.target_state_rel_ag32_init
+  |> Q.GEN`r0` |> Q.SPEC`0w`
+  |> SIMP_RULE std_ss[``n2w ZERO :word32`` |> SIMP_CONV std_ss [ALT_ZERO] ]
+  |> SIMP_RULE(srw_ss())[EVAL``byte_aligned 0w``, markerTheory.Abbrev_def]
+
 (* TODO: move *)
 val int_toString_num = Q.store_thm("int_toString_num",
   `mlint$toString (&n) = mlnum$toString n`,
@@ -107,8 +117,8 @@ val wordcount_init_memory_words_def = zDefine`
     `;
 
 val wordcount_init_memory_def = Define`
-  wordcount_init_memory r0 (cl, stdin) (k:word32) =
-     get_byte k (EL (w2n (byte_align k - r0) DIV 4) (wordcount_init_memory_words cl stdin)) F`;
+  wordcount_init_memory (cl, stdin) (k:word32) =
+     get_byte k (EL (w2n (byte_align k) DIV 4) (wordcount_init_memory_words cl stdin)) F`;
 
 val LENGTH_wordcount_init_memory_words = Q.store_thm("LENGTH_wordcount_init_memory_words",
   `SUM (MAP strlen cl) + LENGTH cl ≤ cline_size ∧ LENGTH inp ≤ stdin_size ⇒
@@ -133,25 +143,23 @@ val LENGTH_wordcount_init_memory_words = Q.store_thm("LENGTH_wordcount_init_memo
 
 val wordcount_machine_config_def = Define`
   wordcount_machine_config =
-    ag32_machine_config (THE config.ffi_names) (LENGTH code) (LENGTH data)`;
+    ag32_machine_config (THE config.ffi_names) (LENGTH code) (LENGTH data) 0w`;
 
 val wordcount_machine_config_halt_pc =
-  ``(wordcount_machine_config r0).halt_pc``
+  ``(wordcount_machine_config).halt_pc``
   |> EVAL |> SIMP_RULE(srw_ss())[ffi_names]
 
 val wordcount_machine_config_ccache_pc =
-  ``(wordcount_machine_config r0).ccache_pc``
+  ``(wordcount_machine_config).ccache_pc``
   |> EVAL |> SIMP_RULE(srw_ss())[ffi_names]
 
 val wordcount_init_memory_startup = Q.store_thm("wordcount_init_memory_startup",
-  `byte_aligned r0 ∧ n < LENGTH wordcount_startup_code ⇒
-   (wordcount_init_memory r0 inputs (r0 + (n2w n)) =
+  `n < LENGTH wordcount_startup_code ⇒
+   (wordcount_init_memory inputs (n2w n) =
     EL n wordcount_startup_code)`,
   Cases_on`inputs`
   \\ strip_tac
   \\ simp[wordcount_init_memory_def]
-  \\ fs[alignmentTheory.byte_aligned_def, alignmentTheory.byte_align_def]
-  \\ simp[align_add_aligned_gen]
   \\ Q.ISPECL_THEN[`n`,`F`,`wordcount_startup_code`]mp_tac
        (Q.GEN`i`(INST_TYPE[alpha|->``:32``]get_byte_EL_words_of_bytes))
   \\ simp[bytes_in_word_def,LENGTH_wordcount_startup_code]
@@ -160,81 +168,39 @@ val wordcount_init_memory_startup = Q.store_thm("wordcount_init_memory_startup",
   \\ simp[wordcount_init_memory_words_def]
   \\ rewrite_tac[GSYM APPEND_ASSOC]
   \\ DEP_REWRITE_TAC [EL_APPEND1]
+  \\ simp[LENGTH_words_of_bytes_wordcount_startup_code]
+  \\ fs[LENGTH_wordcount_startup_code, DIV_LT_X]
+  \\ fs[alignmentTheory.align_w2n]
+  \\ DEP_REWRITE_TAC[LESS_MOD]
+  \\ fs[]
   \\ conj_tac
-  >- (
-    simp[LENGTH_words_of_bytes_wordcount_startup_code]
-    \\ fs[LENGTH_wordcount_startup_code, DIV_LT_X]
-    \\ fs[alignmentTheory.align_w2n]
-    \\ DEP_REWRITE_TAC[LESS_MOD]
-    \\ fs[]
-    \\ conj_tac
-    \\ irule IMP_MULT_DIV_LESS
-    \\ fs[] )
-  \\ `r0 + n2w n = n2w n + byte_align r0`
-  by (
-    simp[alignmentTheory.byte_align_def, align_add_aligned_gen]
-    \\ fs[alignmentTheory.aligned_def] )
-  \\ pop_assum SUBST1_TAC
-  \\ DEP_REWRITE_TAC[data_to_word_memoryProofTheory.get_byte_byte_align]
-  \\ EVAL_TAC);
+  \\ irule IMP_MULT_DIV_LESS
+  \\ fs[] );
 
-(*
-(* TODO: use get_mem_word in this theorem *)
-val hello_init_memory_halt = Q.store_thm("hello_init_memory_halt",
-  `byte_aligned r0 ∧
-   (pc = (hello_machine_config r0).halt_pc) ∧
+val wordcount_init_memory_halt = Q.store_thm("wordcount_init_memory_halt",
+  `(pc = wordcount_machine_config.halt_pc) ∧
    SUM (MAP strlen cl) + LENGTH cl ≤ cline_size ∧ LENGTH inp ≤ stdin_size
   ⇒
-   ((hello_init_memory r0 (cl,inp) (pc + 3w) @@
-    ((hello_init_memory r0 (cl,inp) (pc + 2w) @@
-      ((hello_init_memory r0 (cl,inp) (pc + 1w) @@
-        hello_init_memory r0 (cl,inp) (pc)) : word16)) : word24)) =
+  (get_mem_word (wordcount_init_memory (cl,inp)) pc =
     Encode (Jump (fAdd, 0w, Imm 0w)))`,
   strip_tac
   \\ qpat_x_assum`pc = _`(assume_tac o ONCE_REWRITE_RULE[GSYM markerTheory.Abbrev_def])
-  \\ simp[hello_init_memory_def]
-  \\ fs[alignmentTheory.byte_aligned_def, alignmentTheory.byte_align_def]
-  \\ `aligned 2 pc`
+  \\ qspecl_then[`cl`,`inp`]mp_tac wordcount_init_memory_words_def
+  \\ rewrite_tac[GSYM APPEND_ASSOC, ag32_ffi_jumps_def]
+  \\ qmatch_goalsub_abbrev_tac`ls ++ (words_of_bytes F code ++ _)`
+  \\ qmatch_goalsub_abbrev_tac`ls ++ lr`
+  \\ rewrite_tac[APPEND_ASSOC]
+  \\ qmatch_goalsub_abbrev_tac`ll ++ ls ++ lr`
+  \\ strip_tac
+  \\ qspecl_then[`wordcount_init_memory (cl,inp)`,`0`]mp_tac(Q.GENL[`m`,`k`,`off`]get_mem_word_get_byte)
+  \\ simp[]
+  \\ `4 * LENGTH ll = w2n pc`
   by (
-    simp[Abbr`pc`, hello_machine_config_halt_pc]
-    \\ (alignmentTheory.aligned_add_sub_cor
-        |> SPEC_ALL |> UNDISCH |> CONJUNCT1 |> DISCH_ALL
-        |> irule)
-    \\ simp[]
-    \\ EVAL_TAC )
-  \\ simp[align_add_aligned_gen]
-  \\ simp[Abbr`pc`]
-  \\ rewrite_tac[hello_machine_config_halt_pc]
-  \\ qmatch_goalsub_abbrev_tac`r0 + x`
-  \\ `align 2 (r0 + x) = r0 + x` by fs[alignmentTheory.aligned_def, hello_machine_config_halt_pc]
-  \\ `r0 + x = byte_align (r0 + x)` by fs[alignmentTheory.byte_align_def]
-  \\ qhdtm_x_assum`align`SUBST_ALL_TAC
-  \\ simp_tac(srw_ss())[]
-  \\ pop_assum SUBST_ALL_TAC
-  \\ once_rewrite_tac[WORD_ADD_COMM]
-  \\ DEP_REWRITE_TAC[data_to_word_memoryProofTheory.get_byte_byte_align]
-  \\ conj_tac >- EVAL_TAC
-  \\ DEP_REWRITE_TAC[
-       data_to_word_memoryProofTheory.get_byte_byte_align
-       |> Q.GEN`a'` |> Q.SPEC`0w` |> SIMP_RULE(srw_ss())[]]
-  \\ conj_tac >- EVAL_TAC
-  \\ DEP_REWRITE_TAC[w2n_add]
-  \\ DEP_REWRITE_TAC[ADD_DIV_RWT]
-  \\ conj_tac
-  >- ( simp[Abbr`x`] \\ EVAL_TAC )
-  \\ conj_tac
-  >- ( simp[Abbr`x`,LENGTH_data] \\ EVAL_TAC )
-  \\ qmatch_goalsub_abbrev_tac`_ = h`
-  \\ `∃l1 l2. (hello_init_memory_words cl inp = l1 ++ l2) ∧
-              (LENGTH l1 = w2n x DIV 4) ∧
-              (l2 <> [] ∧ (HD l2 = h))` by (
-    simp[hello_init_memory_words_def, ag32_ffi_jumps_def]
-    \\ qmatch_goalsub_abbrev_tac`l1 ++ halt_jump_ag32_code ++ _ ++ _`
-    \\ qexists_tac`l1`
-    \\ simp[halt_jump_ag32_code_def]
-    \\ simp[Abbr`l1`,Abbr`x`]
-    \\ simp[LENGTH_words_of_bytes_hello_startup_code, LENGTH_words_of_bytes, LENGTH_FLAT, bitstringTheory.length_pad_right]
-    \\ simp[LENGTH_data, LENGTH_code]
+    simp[Abbr`ll`, LENGTH_words_of_bytes_wordcount_startup_code,
+         LENGTH_wordcount_startup_code, startup_code_size_def,
+         heap_size_def, output_buffer_size_def, ccache_jump_ag32_code_def,
+         LENGTH_ag32_ffi_code]
+    \\ simp[LENGTH_words_of_bytes, LENGTH_FLAT, bitstringTheory.length_pad_right]
     \\ simp[MAP_MAP_o, o_DEF, ADD1, ffi_names, SUM_MAP_PLUS]
     \\ simp[Q.ISPEC`λx. 1n`SUM_MAP_K |> SIMP_RULE(srw_ss())[]]
     \\ qmatch_goalsub_abbrev_tac`MIN 1 (cz MOD _)` \\ `cz = stdin_size` by ( simp[Abbr`cz`] )
@@ -243,69 +209,43 @@ val hello_init_memory_halt = Q.store_thm("hello_init_memory_halt",
     \\ qmatch_goalsub_abbrev_tac`MIN 1 (sz MOD _)` \\ `sz = cline_size` by ( simp[Abbr`sz`] )
     \\ qpat_x_assum`Abbrev(sz = _)`kall_tac \\ pop_assum SUBST_ALL_TAC
     \\ simp[cline_size_def, bytes_in_word_def]
-    \\ simp[LENGTH_ag32_ffi_code]
-    \\ simp[LENGTH_hello_startup_code, startup_code_size_def, heap_size_def, output_buffer_size_def]
-    \\ EVAL_TAC)
-  \\ simp[EL_APPEND_EQN]
-  \\ EVAL_TAC \\ simp[]
-  \\ blastLib.BBLAST_TAC );
+    \\ simp[mk_jump_ag32_code_def]
+    \\ simp[Abbr`pc`] \\ EVAL_TAC \\ simp[ffi_names])
+  \\ impl_tac
+  >- (
+    simp[wordcount_init_memory_def, Abbr`ls`]
+    \\ EVAL_TAC
+    \\ reverse conj_asm1_tac
+    >- decide_tac
+    \\ simp[Abbr`pc`]
+    \\ EVAL_TAC
+    \\ simp[ffi_names] )
+  \\ simp[Abbr`ls`, halt_jump_ag32_code_def]);
 
-(* TODO: use get_mem_word in this theorem *)
-val hello_init_memory_ccache = Q.store_thm("hello_init_memory_ccache",
-  `byte_aligned r0 ∧
-   (pc = (hello_machine_config r0).ccache_pc) ∧
+val wordcount_init_memory_ccache = Q.store_thm("wordcount_init_memory_ccache",
+  `(pc = wordcount_machine_config.ccache_pc) ∧
    SUM (MAP strlen cl) + LENGTH cl ≤ cline_size ∧ LENGTH inp ≤ stdin_size
   ⇒
-   ((hello_init_memory r0 (cl,inp) (pc + 3w) @@
-    ((hello_init_memory r0 (cl,inp) (pc + 2w) @@
-      ((hello_init_memory r0 (cl,inp) (pc + 1w) @@
-        hello_init_memory r0 (cl,inp) (pc)) : word16)) : word24)) =
+   (get_mem_word (wordcount_init_memory (cl,inp)) pc =
     Encode (Jump (fSnd, 0w, Reg 0w)))`,
   strip_tac
   \\ qpat_x_assum`pc = _`(assume_tac o ONCE_REWRITE_RULE[GSYM markerTheory.Abbrev_def])
-  \\ simp[hello_init_memory_def]
-  \\ fs[alignmentTheory.byte_aligned_def, alignmentTheory.byte_align_def]
-  \\ `aligned 2 pc`
+  \\ qspecl_then[`cl`,`inp`]mp_tac wordcount_init_memory_words_def
+  \\ rewrite_tac[GSYM APPEND_ASSOC, ag32_ffi_jumps_def]
+  \\ qmatch_goalsub_abbrev_tac`ls ++ (halt_jump_ag32_code ++ _)`
+  \\ qmatch_goalsub_abbrev_tac`ls ++ lr`
+  \\ rewrite_tac[APPEND_ASSOC]
+  \\ qmatch_goalsub_abbrev_tac`ll ++ ls ++ lr`
+  \\ strip_tac
+  \\ qspecl_then[`wordcount_init_memory (cl,inp)`,`0`]mp_tac(Q.GENL[`m`,`k`,`off`]get_mem_word_get_byte)
+  \\ simp[]
+  \\ `4 * LENGTH ll = w2n pc`
   by (
-    simp[Abbr`pc`, hello_machine_config_ccache_pc]
-    \\ (alignmentTheory.aligned_add_sub_cor
-        |> SPEC_ALL |> UNDISCH |> CONJUNCT1 |> DISCH_ALL
-        |> irule)
-    \\ simp[]
-    \\ EVAL_TAC )
-  \\ simp[align_add_aligned_gen]
-  \\ simp[Abbr`pc`]
-  \\ rewrite_tac[hello_machine_config_ccache_pc]
-  \\ qmatch_goalsub_abbrev_tac`r0 + x`
-  \\ `align 2 (r0 + x) = r0 + x` by fs[alignmentTheory.aligned_def, hello_machine_config_ccache_pc]
-  \\ `r0 + x = byte_align (r0 + x)` by fs[alignmentTheory.byte_align_def]
-  \\ qhdtm_x_assum`align`SUBST_ALL_TAC
-  \\ simp_tac(srw_ss())[]
-  \\ pop_assum SUBST_ALL_TAC
-  \\ once_rewrite_tac[WORD_ADD_COMM]
-  \\ DEP_REWRITE_TAC[data_to_word_memoryProofTheory.get_byte_byte_align]
-  \\ conj_tac >- EVAL_TAC
-  \\ DEP_REWRITE_TAC[
-       data_to_word_memoryProofTheory.get_byte_byte_align
-       |> Q.GEN`a'` |> Q.SPEC`0w` |> SIMP_RULE(srw_ss())[]]
-  \\ conj_tac >- EVAL_TAC
-  \\ DEP_REWRITE_TAC[w2n_add]
-  \\ DEP_REWRITE_TAC[ADD_DIV_RWT]
-  \\ conj_tac
-  >- ( simp[Abbr`x`] \\ EVAL_TAC )
-  \\ conj_tac
-  >- ( simp[Abbr`x`,LENGTH_data] \\ EVAL_TAC )
-  \\ qmatch_goalsub_abbrev_tac`_ = h`
-  \\ `∃l1 l2. (hello_init_memory_words cl inp = l1 ++ l2) ∧
-              (LENGTH l1 = w2n x DIV 4) ∧
-              (l2 <> [] ∧ (HD l2 = h))` by (
-    simp[hello_init_memory_words_def, ag32_ffi_jumps_def]
-    \\ qmatch_goalsub_abbrev_tac`l1 ++ ccache_jump_ag32_code ++ _ ++ _ ++ _`
-    \\ qexists_tac`l1`
-    \\ simp[ccache_jump_ag32_code_def]
-    \\ simp[Abbr`l1`,Abbr`x`]
-    \\ simp[LENGTH_words_of_bytes_hello_startup_code, LENGTH_words_of_bytes, LENGTH_FLAT, bitstringTheory.length_pad_right]
-    \\ simp[LENGTH_data, LENGTH_code]
+    simp[Abbr`ll`, LENGTH_words_of_bytes_wordcount_startup_code,
+         LENGTH_wordcount_startup_code, startup_code_size_def,
+         heap_size_def, output_buffer_size_def, ccache_jump_ag32_code_def,
+         LENGTH_ag32_ffi_code]
+    \\ simp[LENGTH_words_of_bytes, LENGTH_FLAT, bitstringTheory.length_pad_right]
     \\ simp[MAP_MAP_o, o_DEF, ADD1, ffi_names, SUM_MAP_PLUS]
     \\ simp[Q.ISPEC`λx. 1n`SUM_MAP_K |> SIMP_RULE(srw_ss())[]]
     \\ qmatch_goalsub_abbrev_tac`MIN 1 (cz MOD _)` \\ `cz = stdin_size` by ( simp[Abbr`cz`] )
@@ -314,27 +254,27 @@ val hello_init_memory_ccache = Q.store_thm("hello_init_memory_ccache",
     \\ qmatch_goalsub_abbrev_tac`MIN 1 (sz MOD _)` \\ `sz = cline_size` by ( simp[Abbr`sz`] )
     \\ qpat_x_assum`Abbrev(sz = _)`kall_tac \\ pop_assum SUBST_ALL_TAC
     \\ simp[cline_size_def, bytes_in_word_def]
-    \\ simp[LENGTH_ag32_ffi_code]
-    \\ simp[LENGTH_hello_startup_code, startup_code_size_def, heap_size_def, output_buffer_size_def]
-    \\ EVAL_TAC)
-  \\ simp[EL_APPEND_EQN]
-  \\ EVAL_TAC \\ simp[]
-  \\ blastLib.BBLAST_TAC );
+    \\ simp[mk_jump_ag32_code_def]
+    \\ simp[Abbr`pc`] \\ EVAL_TAC \\ simp[ffi_names])
+  \\ impl_tac
+  >- (
+    simp[wordcount_init_memory_def, Abbr`ls`]
+    \\ EVAL_TAC
+    \\ reverse conj_asm1_tac
+    >- decide_tac
+    \\ simp[Abbr`pc`]
+    \\ EVAL_TAC
+    \\ simp[ffi_names] )
+  \\ simp[Abbr`ls`, ccache_jump_ag32_code_def]);
 
-(*
-define the ag32 and asm states
-that obtain after running startup code from ag32 init
-and do the rest of the proof from there
-*)
-
-val hello_init_asm_state_def = Define`
-  hello_init_asm_state r0 input =
+val wordcount_init_asm_state_def = Define`
+  wordcount_init_asm_state input =
     FOLDL (λs i. asm i (s.pc + n2w (LENGTH (ag32_enc i))) s)
       (ag32_init_asm_state
-        (hello_init_memory r0 input)
-        (ag32_startup_addresses r0)
-        r0)
-      (hello_startup_asm_code)`;
+        (wordcount_init_memory input)
+        (ag32_startup_addresses 0w)
+        0w)
+      (wordcount_startup_asm_code)`;
 
 val (asm_tm, mk_asm, dest_asm, is_asm) = HolKernel.syntax_fns3 "asmSem" "asm"
 val (asm_ok_tm, mk_asm_ok, dest_asm_ok, is_asm_ok) = HolKernel.syntax_fns2 "asm" "asm_ok"
@@ -357,7 +297,7 @@ val asm_conv =
       handle HOL_ERR _ => Lib.total (list_of_pair o dest_asm_ok) tm)
     (Redblackmap.mkDict (list_compare Term.compare))
     (fn tm => TypeBase.is_record tm orelse aconv tm T)
-    (Feedback.mk_HOL_ERR "hello_ag32Proof" "asm_conv" "")
+    (Feedback.mk_HOL_ERR "wordcount_ag32Proof" "asm_conv" "")
     bare_asm_conv
 
 fun ag32_enc_conv tm =
@@ -367,21 +307,19 @@ fun ag32_enc_conv tm =
 
 val bytes_in_memory_tac =
   simp[asmSemTheory.bytes_in_memory_def, LENGTH_code, ffi_names]
-  \\ DEP_REWRITE_TAC[hello_init_memory_startup, hello_init_memory_startup |> Q.GEN`n` |> Q.SPEC`0` |> SIMP_RULE(srw_ss())[]]
-  \\ simp[LENGTH_hello_startup_code]
-  \\ rewrite_tac[hello_startup_code_eq] \\ EVAL_TAC
-  \\ Cases_on`r0`
+  \\ DEP_REWRITE_TAC[wordcount_init_memory_startup, wordcount_init_memory_startup |> Q.GEN`n` |> Q.SPEC`0` |> SIMP_RULE(srw_ss())[]]
+  \\ simp[LENGTH_wordcount_startup_code]
+  \\ rewrite_tac[wordcount_startup_code_eq] \\ EVAL_TAC
   \\ fs[word_ls_n2w,word_add_n2w,word_lo_n2w,
         alignmentTheory.byte_aligned_def,
         memory_size_def]
 
 val mem_ok_tac =
-  Cases_on`r0`
-  \\ fs[word_ls_n2w,word_add_n2w,word_lo_n2w,
-        alignmentTheory.byte_aligned_def,
-        word_extract_n2w, memory_size_def,
-        GSYM ALIGNED_eq_aligned, addressTheory.ALIGNED_n2w,
-        bitTheory.BITS_ZERO3 ]
+  fs[word_ls_n2w,word_add_n2w,word_lo_n2w,
+     alignmentTheory.byte_aligned_def,
+     word_extract_n2w, memory_size_def,
+     GSYM ALIGNED_eq_aligned, addressTheory.ALIGNED_n2w,
+     bitTheory.BITS_ZERO3 ]
 
 val mem_word_tac =
     rw[data_to_word_memoryProofTheory.word_of_bytes_def,
@@ -392,30 +330,29 @@ val mem_word_tac =
        EVAL``ffi_jumps_offset``]
     \\ blastLib.BBLAST_TAC
 
-val _ = temp_overload_on("hello_asm_state0",
+val _ = temp_overload_on("wordcount_asm_state0",
   ``(ag32_init_asm_state
-      (hello_init_memory r0 (cl,inp))
-      (ag32_startup_addresses r0)
-      r0)``);
+      (wordcount_init_memory (cl,inp))
+      (ag32_startup_addresses 0w)
+      0w)``);
 
-val hello_init_asm_state_asm_step = Q.store_thm("hello_init_asm_state_asm_step",
-  `byte_aligned r0 ∧ w2n r0 + memory_size < dimword(:32) ∧
-   SUM (MAP strlen cl) + LENGTH cl ≤ cline_size ∧
+val wordcount_init_asm_state_asm_step = Q.store_thm("wordcount_init_asm_state_asm_step",
+  `SUM (MAP strlen cl) + LENGTH cl ≤ cline_size ∧
    LENGTH inp ≤ stdin_size ⇒
    let tr =
     (steps (λs i. asm i (s.pc + n2w (LENGTH (ag32_enc i))) s)
-      hello_asm_state0
-      hello_startup_asm_code) in
-   steps_rel (asm_step (ag32_target.config)) hello_asm_state0 tr ∧
-   let final_st = LAST (hello_asm_state0::(MAP SND tr)) in
+      wordcount_asm_state0
+      wordcount_startup_asm_code) in
+   steps_rel (asm_step (ag32_target.config)) wordcount_asm_state0 tr ∧
+   let final_st = LAST (wordcount_asm_state0::(MAP SND tr)) in
    let ffi_names = THE config.ffi_names in
    let num_ffis = LENGTH ffi_names in
-     (final_st.pc = r0 + n2w (code_start_offset num_ffis)) ∧
+     (final_st.pc = n2w (code_start_offset num_ffis)) ∧
      (read_bytearray final_st.pc (LENGTH code)
-       (λa. if a ∈ (hello_machine_config r0).prog_addresses then
+       (λa. if a ∈ wordcount_machine_config.prog_addresses then
                SOME (final_st.mem a) else NONE ) = SOME code) ∧
-     let hs = r0 + n2w heap_start_offset in
-     let ds = r0 + n2w (code_start_offset num_ffis + LENGTH code) in
+     let hs = n2w heap_start_offset in
+     let ds = n2w (code_start_offset num_ffis + LENGTH code) in
      (final_st.regs 2 = hs) ∧
      (final_st.regs 4 = hs + n2w heap_size) ∧
      (word_of_bytes F 0w (GENLIST (final_st.mem o ((+) (hs + 0w * 4w)) o n2w) 4) =
@@ -430,11 +367,11 @@ val hello_init_asm_state_asm_step = Q.store_thm("hello_init_asm_state_asm_step",
       ds) ∧
      (∀k. k < 4 * LENGTH data + 4 ⇒
           (final_st.mem (ds + n2w k) =
-           (hello_init_memory r0 (cl,inp)) (ds + n2w k)))`,
+           (wordcount_init_memory (cl,inp)) (ds + n2w k)))`,
   strip_tac
   \\ qho_match_abbrev_tac`LET (λtr. (_ tr) ∧ P (_ tr)) _`
-  \\ rewrite_tac[hello_startup_asm_code_eq,
-                 EVAL``ag32_startup_addresses r0``]
+  \\ rewrite_tac[wordcount_startup_asm_code_eq,
+                 EVAL``ag32_startup_addresses 0w``]
   \\ simp[]
   \\ qmatch_goalsub_abbrev_tac`steps _ _ (i::tr)`
   \\ simp[steps_def, steps_rel_def]
@@ -445,7 +382,7 @@ val hello_init_asm_state_asm_step = Q.store_thm("hello_init_asm_state_asm_step",
   \\ qpat_x_assum`Abbrev (s2 = _)`mp_tac
   \\ CONV_TAC(ONCE_DEPTH_CONV ag32_enc_conv)
   \\ simp [ag32_init_asm_state_def]
-  \\ `ag32_init_asm_regs r0 = (λk. ag32_init_asm_regs r0 k)` by simp[FUN_EQ_THM]
+  \\ `ag32_init_asm_regs (0w:word32) = (λk. ag32_init_asm_regs 0w k)` by simp[FUN_EQ_THM]
   \\ pop_assum SUBST1_TAC
   \\ simp[ag32_init_asm_regs_def]
   \\ CONV_TAC (PATH_CONV "lrrr" asm_conv)
@@ -480,28 +417,18 @@ val hello_init_asm_state_asm_step = Q.store_thm("hello_init_asm_state_asm_step",
   \\ simp_tac (std_ss++LET_ss) [Abbr`s2`,Abbr`P`]
   \\ conj_tac >- (EVAL_TAC \\ simp[ffi_names])
   \\ conj_tac >- (
-    simp[hello_machine_config_def,
+    simp[wordcount_machine_config_def,
          lab_to_targetTheory.ffi_offset_def,
          heap_size_def, memory_size_def, LENGTH_data,
          ag32_targetTheory.ag32_target_def]
     \\ match_mp_tac data_to_word_assignProofTheory.IMP_read_bytearray_GENLIST
     \\ simp[]
     \\ gen_tac \\ strip_tac
-    \\ qpat_x_assum`_ < dimword _`mp_tac
     \\ CONV_TAC(LAND_CONV EVAL)
-    \\ CONV_TAC(PATH_CONV"rlr" EVAL)
-    \\ Cases_on`r0`
     \\ fs[word_add_n2w, word_ls_n2w, word_lo_n2w, LENGTH_code, LENGTH_data, ffi_names]
-    \\ strip_tac
-    \\ rewrite_tac[hello_init_memory_def]
+    \\ rewrite_tac[wordcount_init_memory_def]
     \\ qmatch_goalsub_abbrev_tac`i + k`
-    \\ `byte_aligned ((n2w k):word32)` by(
-      simp[Abbr`k`, GSYM word_add_n2w, alignmentTheory.byte_aligned_def]
-      \\ (alignmentTheory.aligned_add_sub_cor
-          |> SPEC_ALL |> UNDISCH |> CONJUNCT1 |> DISCH_ALL
-          |> irule)
-      \\ fs[alignmentTheory.byte_aligned_def]
-      \\ EVAL_TAC )
+    \\ `byte_aligned ((n2w k):word32)` by( simp[Abbr`k`] \\ EVAL_TAC )
     \\ `n2w k = byte_align ((n2w k):word32)`
     by (
       fs[alignmentTheory.byte_aligned_def,
@@ -519,10 +446,6 @@ val hello_init_asm_state_asm_step = Q.store_thm("hello_init_asm_state_asm_step",
       \\ fs[alignmentTheory.byte_aligned_def] )
     \\ once_asm_rewrite_tac[]
     \\ qunabbrev_tac`k`
-    \\ rewrite_tac[WORD_ADD_SUB_SYM]
-    \\ rewrite_tac[GSYM word_add_n2w]
-    \\ rewrite_tac[WORD_ADD_ASSOC]
-    \\ rewrite_tac[WORD_SUB_ADD]
     \\ DEP_REWRITE_TAC[w2n_add]
     \\ conj_tac
     >- (
@@ -536,11 +459,11 @@ val hello_init_asm_state_asm_step = Q.store_thm("hello_init_asm_state_asm_step",
       \\ irule IMP_MULT_DIV_LESS
       \\ fs[] )
     \\ simp[ADD_DIV_RWT]
-    \\ rewrite_tac[hello_init_memory_words_def]
+    \\ rewrite_tac[wordcount_init_memory_words_def]
     \\ rewrite_tac[GSYM APPEND_ASSOC] \\ DEP_ONCE_REWRITE_TAC[EL_APPEND2]
-    \\ simp[LENGTH_words_of_bytes_hello_startup_code]
+    \\ simp[LENGTH_words_of_bytes_wordcount_startup_code]
     \\ rewrite_tac[GSYM APPEND_ASSOC] \\ DEP_ONCE_REWRITE_TAC[EL_APPEND2]
-    \\ simp[LENGTH_hello_startup_code, startup_code_size_def]
+    \\ simp[LENGTH_wordcount_startup_code, startup_code_size_def]
     \\ simp[EL_CONS, PRE_SUB1]
     \\ rewrite_tac[GSYM APPEND_ASSOC] \\ DEP_ONCE_REWRITE_TAC[EL_APPEND2]
     \\ simp[LENGTH_words_of_bytes, bitstringTheory.length_pad_right, LENGTH_FLAT, bytes_in_word_def, MAP_MAP_o, o_DEF, ADD1, SUM_MAP_PLUS]
@@ -601,40 +524,38 @@ val hello_init_asm_state_asm_step = Q.store_thm("hello_init_asm_state_asm_step",
   \\ simp_tac std_ss [asmSemTheory.asm_state_accfupds]
   \\ simp[LENGTH_code,ffi_names,EVAL``code_start_offset num_ffis``,LENGTH_data]
   \\ gen_tac \\ strip_tac
-  \\ Cases_on`r0` \\ fs[memory_size_def]
   \\ rewrite_tac[word_add_n2w] \\ rw[]);
 
-val hello_init_asm_state_RTC_asm_step = Q.store_thm("hello_init_asm_state_RTC_asm_step",
-  `byte_aligned r0 ∧ w2n r0 + memory_size < dimword(:32) ∧
-   SUM (MAP strlen cl) + LENGTH cl ≤ cline_size ∧
+val wordcount_init_asm_state_RTC_asm_step = Q.store_thm("wordcount_init_asm_state_RTC_asm_step",
+  `SUM (MAP strlen cl) + LENGTH cl ≤ cline_size ∧
    LENGTH inp ≤ stdin_size
   ⇒
-   (λx y. ∃i. asm_step ag32_config x i y)^* hello_asm_state0 (hello_init_asm_state r0 (cl,inp)) ∧
+   (λx y. ∃i. asm_step ag32_config x i y)^* wordcount_asm_state0 (wordcount_init_asm_state (cl,inp)) ∧
    let ffi_names = THE config.ffi_names in
    let num_ffis = LENGTH ffi_names in
-   let hs = r0 + n2w heap_start_offset in
-   let ds = r0 + n2w (code_start_offset num_ffis + LENGTH code) in
-   ((hello_init_asm_state r0 (cl,inp)).pc = r0 + n2w (code_start_offset num_ffis)) ∧
-   (read_bytearray (hello_init_asm_state r0 (cl,inp)).pc (LENGTH code)
-      (λa. if a ∈ (hello_machine_config r0).prog_addresses then SOME ((hello_init_asm_state r0 (cl,inp)).mem a) else NONE)
+   let hs = n2w heap_start_offset in
+   let ds = n2w (code_start_offset num_ffis + LENGTH code) in
+   ((wordcount_init_asm_state (cl,inp)).pc = n2w (code_start_offset num_ffis)) ∧
+   (read_bytearray (wordcount_init_asm_state (cl,inp)).pc (LENGTH code)
+      (λa. if a ∈ wordcount_machine_config.prog_addresses then SOME ((wordcount_init_asm_state (cl,inp)).mem a) else NONE)
       = SOME code) ∧
-    ((hello_init_asm_state r0 (cl,inp)).regs 2 = hs) ∧
-    ((hello_init_asm_state r0 (cl,inp)).regs 4 = hs + n2w heap_size) ∧
-    (word_of_bytes F 0w (GENLIST ((hello_init_asm_state r0 (cl,inp)).mem o ((+)(hs + 0w * 4w)) o n2w) 4)
+    ((wordcount_init_asm_state (cl,inp)).regs 2 = hs) ∧
+    ((wordcount_init_asm_state (cl,inp)).regs 4 = hs + n2w heap_size) ∧
+    (word_of_bytes F 0w (GENLIST ((wordcount_init_asm_state (cl,inp)).mem o ((+)(hs + 0w * 4w)) o n2w) 4)
      = ds) ∧
-    (word_of_bytes F 0w (GENLIST ((hello_init_asm_state r0 (cl,inp)).mem o ((+)(hs + 1w * 4w)) o n2w) 4)
+    (word_of_bytes F 0w (GENLIST ((wordcount_init_asm_state (cl,inp)).mem o ((+)(hs + 1w * 4w)) o n2w) 4)
      = ds + n2w (4 * LENGTH data)) ∧
-    (word_of_bytes F 0w (GENLIST ((hello_init_asm_state r0 (cl,inp)).mem o ((+)(hs + 2w * 4w)) o n2w) 4)
+    (word_of_bytes F 0w (GENLIST ((wordcount_init_asm_state (cl,inp)).mem o ((+)(hs + 2w * 4w)) o n2w) 4)
      = ds + n2w (4 * LENGTH data)) ∧
-    (word_of_bytes F 0w (GENLIST ((hello_init_asm_state r0 (cl,inp)).mem o ((+)(hs + 3w * 4w)) o n2w) 4)
+    (word_of_bytes F 0w (GENLIST ((wordcount_init_asm_state (cl,inp)).mem o ((+)(hs + 3w * 4w)) o n2w) 4)
      = ds) ∧
-    (word_of_bytes F 0w (GENLIST ((hello_init_asm_state r0 (cl,inp)).mem o ((+)(hs + 4w * 4w)) o n2w) 4)
+    (word_of_bytes F 0w (GENLIST ((wordcount_init_asm_state (cl,inp)).mem o ((+)(hs + 4w * 4w)) o n2w) 4)
      = ds) ∧
     (∀k. k < 4 * LENGTH data + 4 ⇒
-      ((hello_init_asm_state r0 (cl,inp)).mem (ds + n2w k) =
-       hello_init_memory r0 (cl,inp) (ds + n2w k)))`,
+      ((wordcount_init_asm_state (cl,inp)).mem (ds + n2w k) =
+       wordcount_init_memory (cl,inp) (ds + n2w k)))`,
   disch_then assume_tac
-  \\ mp_tac (UNDISCH hello_init_asm_state_asm_step)
+  \\ mp_tac (UNDISCH wordcount_init_asm_state_asm_step)
   \\ simp[]
   \\ strip_tac
   \\ drule steps_rel_LRC
@@ -643,158 +564,112 @@ val hello_init_asm_state_RTC_asm_step = Q.store_thm("hello_init_asm_state_RTC_as
   \\ simp[]
   \\ strip_tac
   \\ drule NRC_RTC
-  \\ fs[LAST_MAP_SND_steps_FOLDL, GSYM hello_init_asm_state_def]
+  \\ fs[LAST_MAP_SND_steps_FOLDL, GSYM wordcount_init_asm_state_def]
   \\ fs[ag32_targetTheory.ag32_target_def]);
 
-val target_state_rel_hello_init_asm_state = Q.store_thm("target_state_rel_hello_init_asm_state",
-  `Abbrev (r0 = n2w ZERO) ∧ byte_aligned r0 ∧ w2n r0 + memory_size < dimword (:32) ∧
-   SUM (MAP strlen cl) + LENGTH cl ≤ cline_size ∧
+val target_state_rel_wordcount_init_asm_state = Q.store_thm("target_state_rel_wordcount_init_asm_state",
+  `SUM (MAP strlen cl) + LENGTH cl ≤ cline_size ∧
    LENGTH inp ≤ stdin_size ∧
-   is_ag32_init_state (hello_init_memory r0 (cl,inp)) ms ⇒
-   ∃n. target_state_rel ag32_target (hello_init_asm_state r0 (cl,inp)) (FUNPOW Next n ms) ∧
+   is_ag32_init_state (wordcount_init_memory (cl,inp)) ms ⇒
+   ∃n. target_state_rel ag32_target (wordcount_init_asm_state (cl,inp)) (FUNPOW Next n ms) ∧
        ((FUNPOW Next n ms).io_events = ms.io_events) ∧
-       (∀x. x ∉ (ag32_startup_addresses r0) ⇒
+       (∀x. x ∉ (ag32_startup_addresses 0w) ⇒
          ((FUNPOW Next n ms).MEM x = ms.MEM x))`,
   strip_tac
-  \\ imp_res_tac hello_init_asm_state_RTC_asm_step
+  \\ imp_res_tac wordcount_init_asm_state_RTC_asm_step
   \\ drule (GEN_ALL target_state_rel_ag32_init)
   \\ rveq
-  \\ disch_then drule
-  \\ disch_then drule
   \\ qmatch_goalsub_abbrev_tac`_ ∉ md`
   \\ disch_then(qspec_then`md`assume_tac)
   \\ drule (GEN_ALL RTC_asm_step_ag32_target_state_rel_io_events)
-  \\ simp[EVAL``(ag32_init_asm_state m md r0).mem_domain``]);
+  \\ simp[EVAL``(ag32_init_asm_state m md 0w).mem_domain``]);
 
-val hello_startup_clock_def =
-  new_specification("hello_startup_clock_def",["hello_startup_clock"],
-  GEN_ALL (Q.SPEC`ms0`(Q.GEN`ms`target_state_rel_hello_init_asm_state))
+val wordcount_startup_clock_def =
+  new_specification("wordcount_startup_clock_def",["wordcount_startup_clock"],
+  GEN_ALL (Q.SPEC`ms0`(Q.GEN`ms`target_state_rel_wordcount_init_asm_state))
   |> SIMP_RULE bool_ss [GSYM RIGHT_EXISTS_IMP_THM,SKOLEM_THM]);
 
-val hello_good_init_state = Q.store_thm("hello_good_init_state",
-  `Abbrev (r0 = n2w ZERO) ∧ byte_aligned r0 ∧ w2n r0 + memory_size < dimword(:32) ∧
-   SUM (MAP strlen cl) + LENGTH cl ≤ cline_size ∧
+val wordcount_good_init_state = Q.store_thm("wordcount_good_init_state",
+  `SUM (MAP strlen cl) + LENGTH cl ≤ cline_size ∧
    LENGTH inp ≤ stdin_size ∧
-   is_ag32_init_state (hello_init_memory r0 (cl,inp)) ms0 ⇒
+   is_ag32_init_state (wordcount_init_memory (cl,inp)) ms0 ⇒
    ∃io_regs cc_regs.
-   good_init_state (hello_machine_config r0) (FUNPOW Next (hello_startup_clock r0 ms0 inp cl) ms0)
+   good_init_state wordcount_machine_config (FUNPOW Next (wordcount_startup_clock ms0 inp cl) ms0)
      (basis_ffi cl fs) code 0
-     ((hello_init_asm_state r0 (cl,inp)) with mem_domain := (hello_machine_config r0).prog_addresses)
+     ((wordcount_init_asm_state (cl,inp)) with mem_domain := wordcount_machine_config.prog_addresses)
      (λk. Word
-       (word_of_bytes F 0w (GENLIST (λi. (hello_init_asm_state r0 (cl,inp)).mem (k + n2w i)) 4)))
-       ({w | (hello_init_asm_state r0 (cl,inp)).regs 2 <=+ w ∧
-             w <+ (hello_init_asm_state r0 (cl,inp)).regs 4}
-        ∪ {w | r0 + n2w (code_start_offset (LENGTH (THE config.ffi_names)) + LENGTH code) <=+ w ∧
-               w <+ r0 + n2w(code_start_offset (LENGTH (THE config.ffi_names)) + LENGTH code + 4 * LENGTH data) })
+       (word_of_bytes F 0w (GENLIST (λi. (wordcount_init_asm_state (cl,inp)).mem (k + n2w i)) 4)))
+       ({w | (wordcount_init_asm_state (cl,inp)).regs 2 <=+ w ∧
+             w <+ (wordcount_init_asm_state (cl,inp)).regs 4}
+        ∪ {w | n2w (code_start_offset (LENGTH (THE config.ffi_names)) + LENGTH code) <=+ w ∧
+               w <+ n2w(code_start_offset (LENGTH (THE config.ffi_names)) + LENGTH code + 4 * LENGTH data) })
      io_regs
      cc_regs`,
   strip_tac
-  \\ drule hello_startup_clock_def \\ fs[]
+  \\ drule wordcount_startup_clock_def \\ fs[]
   \\ disch_then drule \\ disch_then drule
-  \\ disch_then drule
   \\ strip_tac
   \\ simp[lab_to_targetProofTheory.good_init_state_def,RIGHT_EXISTS_AND_THM]
-  \\ drule hello_init_asm_state_RTC_asm_step
+  \\ mp_tac wordcount_init_asm_state_RTC_asm_step
   \\ impl_tac >- fs[]
   \\ strip_tac
   \\ conj_tac >- (
-    fs[hello_machine_config_def, ag32_machine_config_def]
+    fs[wordcount_machine_config_def, ag32_machine_config_def]
     \\ fs[asmPropsTheory.target_state_rel_def]
     \\ fs[EVAL``ag32_target.get_byte``]
     \\ qx_gen_tac`a` \\ strip_tac
     \\ drule asmPropsTheory.RTC_asm_step_consts
     \\ strip_tac \\ fs[]
-    \\ `hello_asm_state0.mem_domain = ag32_startup_addresses r0` by (
+    \\ `wordcount_asm_state0.mem_domain = ag32_startup_addresses 0w` by (
       fs[ag32_init_asm_state_def] )
     \\ fs[]
-    \\ Cases_on`a ∈ ag32_startup_addresses r0` \\ fs[]
+    \\ Cases_on`a ∈ ag32_startup_addresses 0w` \\ fs[]
     \\ drule asmPropsTheory.RTC_asm_step_outside_mem_domain
     \\ simp[]
     \\ fs[is_ag32_init_state_def]
     \\ simp[ag32_init_asm_state_def])
   \\ conj_tac
   >- (
-    Q.ISPEC_THEN `hello_machine_config r0 with prog_addresses := ag32_startup_addresses r0`
+    Q.ISPEC_THEN `wordcount_machine_config with prog_addresses := ag32_startup_addresses 0w`
       drule (Q.GEN`mc` RTC_asm_step_target_configured)
     \\ simp[lab_to_targetProofTheory.target_configured_def]
     \\ impl_tac >- EVAL_TAC
     \\ strip_tac \\ fs[])
   \\ conj_tac >- (
-    fs[asmPropsTheory.target_state_rel_def, hello_machine_config_def, ag32_machine_config_def] )
+    fs[asmPropsTheory.target_state_rel_def, wordcount_machine_config_def, ag32_machine_config_def] )
   \\ qabbrev_tac`num_ffis = LENGTH (THE config.ffi_names)`
-  \\ `r0 + n2w (code_start_offset num_ffis) && 3w = 0w` by (
+  \\ `n2w (code_start_offset num_ffis) && 3w = 0w:word32` by (
     EVAL_TAC
-    \\ fs[alignmentTheory.aligned_bitwise_and, alignmentTheory.byte_aligned_def, Abbr`num_ffis`, ffi_names]
-    \\ Cases_on`r0`
-    \\ simp[word_add_n2w]
-    \\ once_rewrite_tac[WORD_AND_COMM]
-    \\ rewrite_tac[addressTheory.n2w_and_3]
-    \\ qpat_x_assum`_ = 0w`mp_tac
-    \\ once_rewrite_tac[WORD_AND_COMM]
-    \\ rewrite_tac[addressTheory.n2w_and_3]
-    \\ EVAL_TAC
-    \\ simp[] )
-  \\ `r0 + n2w (code_start_offset num_ffis) && 1w = 0w` by (
+    \\ fs[alignmentTheory.aligned_bitwise_and, alignmentTheory.byte_aligned_def, Abbr`num_ffis`, ffi_names])
+  \\ `n2w (code_start_offset num_ffis) && 1w = 0w:word32` by (
     EVAL_TAC
-    \\ fs[alignmentTheory.aligned_bitwise_and, alignmentTheory.byte_aligned_def, Abbr`num_ffis`, ffi_names]
-    \\ Cases_on`r0`
-    \\ simp[word_add_n2w]
-    \\ once_rewrite_tac[WORD_AND_COMM]
-    \\ rewrite_tac[addressTheory.n2w_and_1]
-    \\ qpat_x_assum`_ && n2w _ = 0w`mp_tac
-    \\ once_rewrite_tac[WORD_AND_COMM]
-    \\ rewrite_tac[addressTheory.n2w_and_3]
-    \\ EVAL_TAC
-    \\ simp[]
-    \\ DEP_ONCE_REWRITE_TAC[LESS_MOD]
-    \\ conj_tac
-    >- (
-      match_mp_tac LESS_LESS_EQ_TRANS
-      \\ qexists_tac`4`
-      \\ simp[MOD_LESS] )
-    \\ strip_tac
-    \\ DEP_ONCE_REWRITE_TAC[LESS_MOD]
-    \\ conj_tac
-    >- (
-      match_mp_tac LESS_LESS_EQ_TRANS
-      \\ qexists_tac`2`
-      \\ simp[MOD_LESS] )
-    \\ fs[MOD_EQ_0_DIVISOR]
-    \\ qexists_tac`2 * d`
-    \\ simp[] )
+    \\ fs[alignmentTheory.aligned_bitwise_and, alignmentTheory.byte_aligned_def, Abbr`num_ffis`, ffi_names])
   \\ conj_tac >- (
     rewrite_tac[lab_to_targetProofTheory.start_pc_ok_def]
-    \\ conj_tac >- (
-      qpat_x_assum`_ < _`mp_tac
-      \\ EVAL_TAC \\ simp[LENGTH_code, LENGTH_data, ffi_names, Abbr`num_ffis`]
-      \\ Cases_on`r0`
-      \\ fs[WORD_LOWER_OR_EQ,WORD_NOT_LOWER,word_add_n2w,word_ls_n2w,word_lo_n2w] )
-    \\ conj_tac >- (
-      qpat_x_assum`_ < _`mp_tac
-      \\ EVAL_TAC \\ simp[LENGTH_code, LENGTH_data, ffi_names, Abbr`num_ffis`]
-      \\ Cases_on`r0`
-      \\ simp[WORD_LOWER_OR_EQ,WORD_NOT_LOWER,word_add_n2w,word_ls_n2w,word_lo_n2w] )
+    \\ conj_tac >- ( EVAL_TAC \\ simp[LENGTH_code, LENGTH_data, ffi_names, Abbr`num_ffis`])
+    \\ conj_tac >- ( EVAL_TAC \\ simp[LENGTH_code, LENGTH_data, ffi_names, Abbr`num_ffis`])
     \\ simp[lab_to_targetTheory.ffi_offset_def]
     \\ conj_tac >- (EVAL_TAC \\ simp[ffi_names,Abbr`num_ffis`])
     \\ conj_tac >- (EVAL_TAC \\ simp[ffi_names,Abbr`num_ffis`] )
     \\ conj_tac >- fs[]
-    \\ rewrite_tac[EVAL``(hello_machine_config r0).ffi_names``]
+    \\ rewrite_tac[EVAL``wordcount_machine_config.ffi_names``]
     \\ fs[ffi_names, Abbr`num_ffis`,lab_to_targetTheory.ffi_offset_def, EVAL``code_start_offset n``]
-    \\ simp[hello_machine_config_def, ffi_names, ag32_machine_config_def]
+    \\ gen_tac \\ CONV_TAC(LAND_CONV(SIMP_CONV(srw_ss())[NUMERAL_LESS_THM]))
+    \\ simp[wordcount_machine_config_def, ffi_names, ag32_machine_config_def]
     \\ EVAL_TAC \\ simp[LENGTH_data, LENGTH_code]
-    \\ Cases_on`r0`
-    \\ fs[WORD_LOWER_OR_EQ,WORD_NOT_LOWER,word_add_n2w,word_ls_n2w,word_lo_n2w,memory_size_def] )
+    \\ strip_tac \\ rveq \\ EVAL_TAC)
   \\ conj_tac >- (
-    qpat_x_assum`_ && 3w = _`mp_tac
-    \\ EVAL_TAC \\ fs[] )
+    imp_res_tac asmPropsTheory.RTC_asm_step_consts
+    \\ qpat_x_assum`_ && 3w = _`mp_tac \\ fs[]
+    \\ simp[ag32_init_asm_state_def] )
   \\ conj_tac >- (
     rw[asmPropsTheory.interference_ok_def]
-    \\ simp[EVAL``(hello_machine_config r0).target``]
-    \\ simp[EVAL``(hello_machine_config r0).next_interfer``] )
+    \\ simp[EVAL``(wordcount_machine_config).target``]
+    \\ simp[EVAL``(wordcount_machine_config).next_interfer``] )
   \\ simp[LEFT_EXISTS_AND_THM]
   \\ conj_tac >- (
     simp[lab_to_targetProofTheory.ffi_interfer_ok_def]
-    \\ simp[hello_machine_config_def, ag32_machine_config_def]
+    \\ simp[wordcount_machine_config_def, ag32_machine_config_def]
     \\ simp[lab_to_targetTheory.ffi_offset_def,LENGTH_data,heap_size_def,Abbr`num_ffis`,ffi_names]
     \\ simp[EVAL``ag32_target.config``,labSemTheory.get_reg_value_def]
     \\ simp[ag32_ffi_interfer_def]
@@ -827,18 +702,14 @@ val hello_good_init_state = Q.store_thm("hello_good_init_state",
         \\ qpat_x_assum`_ ∈ _.mem_domain`mp_tac
         \\ qpat_x_assum`_ = _.mem_domain`(assume_tac o SYM)
         \\ simp[ag32_prog_addresses_def]
-        \\ EVAL_TAC
-        \\ Cases_on`r0` \\ fs[memory_size_def, word_add_n2w, word_ls_n2w, word_lo_n2w] )
+        \\ EVAL_TAC)
       \\ reverse IF_CASES_TAC
       >- (
         rw[APPLY_UPDATE_THM]
         \\ qpat_x_assum`_ ∈ _.mem_domain`mp_tac
         \\ qpat_x_assum`_ = _.mem_domain`(assume_tac o SYM)
         \\ simp[ag32_prog_addresses_def]
-        \\ EVAL_TAC
-        \\ qpat_x_assum`Abbrev(r0 = _)`mp_tac
-        \\ simp[Once ALT_ZERO]
-        \\ strip_tac \\ simp[Abbr`r0`] )
+        \\ EVAL_TAC)
       \\ rw[]
       \\ fs[targetSemTheory.read_ffi_bytearrays_def]
       \\ fs[targetSemTheory.read_ffi_bytearray_def]
@@ -859,20 +730,19 @@ val hello_good_init_state = Q.store_thm("hello_good_init_state",
       \\ fs[EVAL``output_offset``, output_buffer_size_def]
       \\ fs[LENGTH_TAKE_EQ, fsFFITheory.write_def]
       \\ pairarg_tac \\ fs[]
-      \\ Cases_on`r0` \\ fs[memory_size_def, word_add_n2w]
       \\ qpat_x_assum`_ ∈ _.mem_domain`mp_tac
       \\ qpat_x_assum`_ = _.mem_domain`(mp_tac o SYM)
       \\ simp[ag32_prog_addresses_def]
       \\ strip_tac
       \\ CONV_TAC(LAND_CONV EVAL)
-      \\ Cases_on`a` \\ fs[word_ls_n2w, word_lo_n2w]
+      \\ Cases_on`a` \\ fs[word_ls_n2w, word_lo_n2w, word_add_n2w]
       \\ rw[MIN_DEF])
     \\ simp[APPLY_UPDATE_THM]
     \\ rpt strip_tac
     \\ rpt(IF_CASES_TAC \\ simp[labSemTheory.get_reg_value_def]))
   \\ conj_tac >- (
     rw[lab_to_targetProofTheory.ccache_interfer_ok_def,
-       hello_machine_config_def, ag32_machine_config_def,
+       wordcount_machine_config_def, ag32_machine_config_def,
        lab_to_targetTheory.ffi_offset_def, ag32_ccache_interfer_def,
        LENGTH_data, heap_size_def, EVAL``ag32_target.config``]
     \\ qmatch_goalsub_abbrev_tac`0w =+ v0`
@@ -882,7 +752,7 @@ val hello_good_init_state = Q.store_thm("hello_good_init_state",
   \\ conj_asm1_tac >- (
     simp[targetSemTheory.code_loaded_def]
     \\ fs[asmPropsTheory.target_state_rel_def]
-    \\ simp[SIMP_CONV (srw_ss()) [hello_machine_config_def,ag32_machine_config_def]``(hello_machine_config r0).target``]
+    \\ simp[SIMP_CONV (srw_ss()) [wordcount_machine_config_def,ag32_machine_config_def]``(wordcount_machine_config).target``]
     \\ rfs[]
     \\ first_x_assum(CONV_TAC o RAND_CONV o REWR_CONV o SYM)
     \\ AP_TERM_TAC
@@ -890,7 +760,7 @@ val hello_good_init_state = Q.store_thm("hello_good_init_state",
     \\ rw[]
     \\ match_mp_tac EQ_SYM
     \\ fs[EVAL``ag32_target.get_byte``]
-    \\ reverse(Cases_on`a ∈ ag32_startup_addresses r0`) \\ fs[]
+    \\ reverse(Cases_on`a ∈ ag32_startup_addresses 0w`) \\ fs[]
     >- (
       drule asmPropsTheory.RTC_asm_step_outside_mem_domain
       \\ simp[ag32_init_asm_state_def]
@@ -907,19 +777,14 @@ val hello_good_init_state = Q.store_thm("hello_good_init_state",
     \\ qpat_x_assum`_ = _.pc`(assume_tac o SYM) \\ fs[]
     \\ EVAL_TAC
     \\ simp[LENGTH_data,LENGTH_code,Abbr`num_ffis`,ffi_names]
-    \\ Cases_on`r0` \\  fs[word_add_n2w,memory_size_def]
-    \\ Cases \\ fs[word_lo_n2w, word_ls_n2w])
+    \\ Cases \\ fs[word_lo_n2w, word_ls_n2w, word_add_n2w])
   \\ conj_tac >- (
-    qpat_x_assum`_ + _ < _`mp_tac
-    \\ imp_res_tac asmPropsTheory.RTC_asm_step_consts
+    imp_res_tac asmPropsTheory.RTC_asm_step_consts
     \\ fs[LENGTH_data,heap_size_def]
     \\ EVAL_TAC
     \\ simp[SUBSET_DEF, LENGTH_code, LENGTH_data, Abbr`num_ffis`, ffi_names]
-    \\ Cases_on`r0` \\ fs[word_add_n2w]
-    \\ strip_tac
-    \\ simp[GSYM FORALL_AND_THM]
     \\ Cases
-    \\ fs[word_lo_n2w, word_ls_n2w])
+    \\ fs[word_lo_n2w, word_ls_n2w, word_add_n2w])
   \\ conj_tac >- (
     gen_tac
     \\ qmatch_goalsub_abbrev_tac`low <=+ byte_align a`
@@ -930,26 +795,15 @@ val hello_good_init_state = Q.store_thm("hello_good_init_state",
       \\ irule (SIMP_RULE (srw_ss()) [] byte_align_IN_IMP_IN_range)
       \\ simp[Abbr`hi`,Abbr`low`]
       \\ fs[alignmentTheory.byte_aligned_def]
-      \\ rewrite_tac[word_add_n2w, GSYM WORD_ADD_ASSOC]
-      \\ conj_tac
-      \\ (alignmentTheory.aligned_add_sub_cor
-          |> SPEC_ALL |> UNDISCH |> CONJUNCT1 |> DISCH_ALL
-          |> irule)
-      \\ fs[]
       \\ EVAL_TAC )
     \\ disj2_tac
     \\ irule (SIMP_RULE (srw_ss()) [] byte_align_IN_IMP_IN_range)
     \\ simp[heap_size_def,LENGTH_data,LENGTH_code]
     \\ fs[alignmentTheory.byte_aligned_def,Abbr`hi`,heap_size_def]
-    \\ conj_tac
-    \\ (alignmentTheory.aligned_add_sub_cor
-        |> SPEC_ALL |> UNDISCH |> CONJUNCT1 |> DISCH_ALL
-        |> irule)
-    \\ fs[]
     \\ simp[Abbr`num_ffis`,ffi_names]
     \\ EVAL_TAC )
   \\ conj_tac >- (
-    simp[EVAL``(hello_machine_config r0).target.config``]
+    simp[EVAL``(wordcount_machine_config).target.config``]
     \\ Cases
     \\ qmatch_asmsub_rename_tac`i < dimword _`
     \\ `byte_align ((n2w i):word32) <=+ n2w i`
@@ -995,39 +849,38 @@ val hello_good_init_state = Q.store_thm("hello_good_init_state",
     \\ Cases_on`q` \\ fs[] >- metis_tac[] )
   \\ simp[LENGTH_code]);
 
-val is_ag32_machine_config_hello_machine_config = Q.store_thm("is_ag32_machine_config_hello_machine_config",
-  `is_ag32_machine_config (hello_machine_config r0)`,
-  rw[hello_machine_config_def, is_ag32_machine_config_ag32_machine_config]);
+val is_ag32_machine_config_wordcount_machine_config = Q.store_thm("is_ag32_machine_config_wordcount_machine_config",
+  `is_ag32_machine_config wordcount_machine_config`,
+  rw[wordcount_machine_config_def, is_ag32_machine_config_ag32_machine_config]);
 
 val compile_correct_applied =
-  MATCH_MP compile_correct hello_compiled
+  MATCH_MP compile_correct wordcount_compiled
   |> SIMP_RULE(srw_ss())[LET_THM,ml_progTheory.init_state_env_thm,GSYM AND_IMP_INTRO]
-  |> C MATCH_MP hello_not_fail
+  |> C MATCH_MP wordcount_not_fail
   |> C MATCH_MP ag32_backend_config_ok
-  |> REWRITE_RULE[hello_sem_sing,AND_IMP_INTRO]
+  |> REWRITE_RULE[wordcount_sem_sing,AND_IMP_INTRO]
   |> REWRITE_RULE[Once (GSYM AND_IMP_INTRO)]
   |> C MATCH_MP (CONJ(UNDISCH ag32_machine_config_ok)(UNDISCH ag32_init_ok))
   |> DISCH(#1(dest_imp(concl ag32_init_ok)))
-  |> C MATCH_MP is_ag32_machine_config_hello_machine_config
+  |> C MATCH_MP is_ag32_machine_config_wordcount_machine_config
   |> Q.GEN`cbspace` |> Q.SPEC`0`
   |> Q.GEN`data_sp` |> Q.SPEC`0`
 
-val hello_installed = Q.store_thm("hello_installed",
-  `Abbrev (r0 = n2w ZERO) ∧ byte_aligned r0 ∧ w2n r0 + memory_size < dimword (:32) ∧
-   SUM (MAP strlen cl) + LENGTH cl ≤ cline_size ∧
+val wordcount_installed = Q.store_thm("wordcount_installed",
+  `SUM (MAP strlen cl) + LENGTH cl ≤ cline_size ∧
    LENGTH inp ≤ stdin_size ∧
-   is_ag32_init_state (hello_init_memory r0 (cl,inp)) ms0 ⇒
+   is_ag32_init_state (wordcount_init_memory (cl,inp)) ms0 ⇒
    installed code 0 data 0 config.ffi_names (basis_ffi cl fs)
      (heap_regs ag32_backend_config.stack_conf.reg_names)
-     (hello_machine_config r0) (FUNPOW Next (hello_startup_clock r0 ms0 inp cl) ms0)`,
+     (wordcount_machine_config) (FUNPOW Next (wordcount_startup_clock ms0 inp cl) ms0)`,
   disch_then assume_tac
   \\ CONV_TAC(PATH_CONV"llr"EVAL)
   \\ simp[backendProofTheory.installed_def]
   \\ simp[word_list_exists_def, set_sepTheory.SEP_CLAUSES, word_list_def]
-  \\ simp[EVAL``(hello_machine_config r0).target.get_pc``]
-  \\ strip_assume_tac(UNDISCH hello_good_init_state)
+  \\ simp[EVAL``(wordcount_machine_config).target.get_pc``]
+  \\ strip_assume_tac(UNDISCH wordcount_good_init_state)
   \\ fs[]
-  \\ drule hello_init_asm_state_RTC_asm_step
+  \\ mp_tac wordcount_init_asm_state_RTC_asm_step
   \\ impl_tac >- fs[]
   \\ strip_tac
   \\ qmatch_asmsub_abbrev_tac`good_init_state _ _ _ _ _ t`
@@ -1036,42 +889,29 @@ val hello_installed = Q.store_thm("hello_installed",
   \\ qhdtm_x_assum`good_init_state` mp_tac
   \\ rewrite_tac[lab_to_targetProofTheory.good_init_state_def]
   \\ disch_then(assume_tac o el 1 o CONJUNCTS)
-  \\ conj_tac
-  >- (irule byte_aligned_add \\ simp[] \\ EVAL_TAC)
-  \\ conj_tac
-  >- (irule byte_aligned_add \\ simp[]
-      \\ reverse conj_tac >- EVAL_TAC
-      \\ irule byte_aligned_add \\ simp[]
-      \\ EVAL_TAC)
-  \\ conj_tac
-  >- (irule byte_aligned_add \\ simp[ffi_names, LENGTH_code] \\ EVAL_TAC)
-  \\ conj_tac
-  >- (Cases_on`r0`
-      \\ EVAL_TAC
-      \\ fs[memory_size_def, heap_size_def])
-  \\ conj_tac
-  >- ( Cases_on`r0` \\ simp[WORD_LEFT_ADD_DISTRIB] \\ EVAL_TAC )
+  \\ conj_tac >- EVAL_TAC
+  \\ conj_tac >- EVAL_TAC
+  \\ conj_tac >- (simp[ffi_names, LENGTH_code] \\ EVAL_TAC)
+  \\ conj_tac >- EVAL_TAC
+  \\ conj_tac >- EVAL_TAC
   \\ conj_tac
   >- (
     simp[IN_DISJOINT]
-    \\ qpat_x_assum`_ < _`mp_tac
     \\ EVAL_TAC
     \\ simp[LENGTH_code,LENGTH_data,ffi_names]
-    \\ strip_tac
     \\ Cases
-    \\ Cases_on`r0`
     \\ fs[word_add_n2w,word_ls_n2w,word_lo_n2w] )
   \\ conj_tac
   >- ( rw[LENGTH_data, bytes_in_word_def, LENGTH_code, ffi_names] )
   \\ conj_tac >- simp[bytes_in_word_def, GSYM word_add_n2w, word_mul_n2w]
   \\ conj_tac >- (
     fs[asmPropsTheory.target_state_rel_def,
-       hello_machine_config_def, ag32_machine_config_def,
+       wordcount_machine_config_def, ag32_machine_config_def,
        ag32_targetTheory.ag32_target_def]
     \\ simp[bytes_in_word_def, GSYM word_add_n2w, GSYM word_mul_n2w] )
   \\ conj_tac >- (
     fs[asmPropsTheory.target_state_rel_def,
-       hello_machine_config_def,
+       wordcount_machine_config_def,
        ag32_machine_config_def,
        ag32_targetTheory.ag32_target_def]
     \\ simp[bytes_in_word_def, GSYM word_add_n2w, GSYM word_mul_n2w] )
@@ -1079,7 +919,7 @@ val hello_installed = Q.store_thm("hello_installed",
     irule IMP_word_list
     \\ fs[LENGTH_code, LENGTH_data, heap_size_def, bytes_in_word_def,
           memory_size_def, ffi_names, EVAL``code_start_offset n``]
-    \\ Cases_on`r0` \\ fs[word_add_n2w]
+    \\ fs[word_add_n2w]
     \\ simp[EXTENSION,FORALL_PROD,set_sepTheory.IN_fun2set]
     \\ reverse(rw[EQ_IMP_THM])
     \\ fs[word_mul_n2w, word_add_n2w, word_lo_n2w, word_ls_n2w]
@@ -1091,9 +931,6 @@ val hello_installed = Q.store_thm("hello_installed",
           |> SPEC_ALL |> UNDISCH |> CONJUNCT1 |> DISCH_ALL
           |> irule)
       \\ reverse conj_tac >- EVAL_TAC
-      \\ (alignmentTheory.aligned_add_sub_cor
-          |> SPEC_ALL |> UNDISCH |> CONJUNCT1 |> DISCH_ALL
-          |> irule)
       \\ fs[alignmentTheory.byte_aligned_def]
       \\ simp[GSYM word_mul_n2w]
       \\ simp[GSYM ALIGNED_eq_aligned]
@@ -1110,24 +947,13 @@ val hello_installed = Q.store_thm("hello_installed",
       \\ ntac 4 (disch_then kall_tac)
       \\ qmatch_goalsub_abbrev_tac`n + off`
       \\ qmatch_goalsub_abbrev_tac`word_of_bytes _ _ ls`
-      \\ `ls = GENLIST (λi. hello_init_memory (n2w n) (cl,inp) (n2w (4 * (k + (off DIV 4)) + n + i))) 4`
+      \\ `ls = GENLIST (λi. wordcount_init_memory (cl,inp) (n2w (4 * (k + (off DIV 4)) + i))) 4`
       by ( simp[Abbr`ls`,Abbr`off`,LEFT_ADD_DISTRIB] )
       \\ qpat_x_assum`Abbrev(ls = _)`kall_tac
       \\ pop_assum SUBST_ALL_TAC
       \\ simp[Abbr`off`, GSYM word_add_n2w]
-      \\ simp[hello_init_memory_def]
+      \\ simp[wordcount_init_memory_def]
       \\ rewrite_tac[GSYM WORD_ADD_ASSOC]
-      \\ `∀x:word32. get_byte (n2w n + x) = get_byte x`
-      by (
-        simp[Once ADD_COMM]
-        \\ `(n2w n : word32) = byte_align ((n2w n):word32)`
-        by ( fs[alignmentTheory.byte_aligned_def, alignmentTheory.byte_align_def, alignmentTheory.aligned_def] )
-        \\ pop_assum SUBST1_TAC
-        \\ simp[FUN_EQ_THM]
-        \\ rpt gen_tac
-        \\ match_mp_tac data_to_word_memoryProofTheory.get_byte_byte_align
-        \\ EVAL_TAC )
-      \\ simp[]
       \\ `∀(y:word32) x. get_byte (n2w (4 * x) + y) = get_byte y`
       by (
         rw[FUN_EQ_THM]
@@ -1141,23 +967,6 @@ val hello_installed = Q.store_thm("hello_installed",
       \\ simp[]
       \\ pop_assum(qspec_then`0w`mp_tac) \\ simp[]
       \\ disch_then kall_tac
-      \\ `∀x:word32. byte_align (n2w n + x) = byte_align x + n2w n`
-      by (
-        `(n2w n : word32) = byte_align ((n2w n):word32)`
-        by ( fs[alignmentTheory.byte_aligned_def, alignmentTheory.byte_align_def, alignmentTheory.aligned_def] )
-        \\ fs[alignmentTheory.byte_aligned_def, alignmentTheory.byte_align_def]
-        \\ gen_tac
-        \\ once_rewrite_tac[WORD_ADD_COMM]
-        \\ DEP_REWRITE_TAC[align_add_aligned_gen]
-        \\ simp[] )
-      \\ rewrite_tac[GSYM WORD_ADD_ASSOC]
-      \\ simp[]
-      \\ rewrite_tac[GSYM WORD_ADD_ASSOC]
-      \\ qmatch_goalsub_abbrev_tac`(_:word32) + zz`
-      \\ `zz = 0w`
-      by ( simp[Abbr`zz`, word_add_n2w] )
-      \\ qpat_x_assum`Abbrev(zz = _)`kall_tac
-      \\ rw[]
       \\ `∀y x. byte_align (n2w (4 * x) + y) = n2w (4 * x) + byte_align y : word32`
       by (
         rw[]
@@ -1176,12 +985,12 @@ val hello_installed = Q.store_thm("hello_installed",
       \\ simp[MULT_DIV]
       \\ qmatch_goalsub_abbrev_tac`get_byte _ mm`
       \\ pop_assum mp_tac
-      \\ rewrite_tac[hello_init_memory_words_def]
+      \\ rewrite_tac[wordcount_init_memory_words_def]
       \\ DEP_REWRITE_TAC[EL_APPEND2]
       \\ qmatch_goalsub_abbrev_tac`ll ≤ _`
       \\ pop_assum mp_tac
-      \\ simp[LENGTH_words_of_bytes_hello_startup_code,LENGTH_ag32_ffi_code,heap_size_def,
-              output_buffer_size_def,startup_code_size_def,LENGTH_hello_startup_code,
+      \\ simp[LENGTH_words_of_bytes_wordcount_startup_code,LENGTH_ag32_ffi_code,heap_size_def,
+              output_buffer_size_def,startup_code_size_def,LENGTH_wordcount_startup_code,
               LENGTH_ag32_ffi_jumps, ffi_names]
       \\ simp[LENGTH_words_of_bytes, bitstringTheory.length_pad_right, LENGTH_code,
               bytes_in_word_def, LENGTH_FLAT, MAP_MAP_o, o_DEF, ADD1, SUM_MAP_PLUS,
@@ -1210,8 +1019,8 @@ val hello_installed = Q.store_thm("hello_installed",
          addressTheory.ALIGNED_n2w]
       \\ fs[MOD_EQ_0_DIVISOR] \\ rfs[]
       \\ fs[Abbr`l`] \\ rveq
-      \\ qmatch_asmsub_abbrev_tac`4 * d + (p + m) = 4 * q`
-      \\ qexists_tac`(q - d - m DIV 4)`
+      \\ qmatch_asmsub_abbrev_tac`p + m = 4 * d`
+      \\ qexists_tac`(d - m DIV 4)`
       \\ simp[Abbr`m`])
     \\ qexists_tac`d`
     \\ simp[]
@@ -1226,24 +1035,13 @@ val hello_installed = Q.store_thm("hello_installed",
     \\ `d < LENGTH data` by ( simp[LENGTH_data] ) \\ simp[EL_MAP]
     \\ qmatch_goalsub_abbrev_tac`n + off`
     \\ qmatch_goalsub_abbrev_tac`word_of_bytes _ _ ls`
-    \\ `ls = GENLIST (λi. hello_init_memory (n2w n) (cl,inp) (n2w (4 * (d + (off DIV 4)) + n + i))) 4`
+    \\ `ls = GENLIST (λi. wordcount_init_memory (cl,inp) (n2w (4 * (d + (off DIV 4)) + i))) 4`
     by ( simp[Abbr`ls`,Abbr`off`,LEFT_ADD_DISTRIB] )
     \\ qpat_x_assum`Abbrev(ls = _)`kall_tac
     \\ pop_assum SUBST_ALL_TAC
     \\ simp[Abbr`off`, GSYM word_add_n2w]
-    \\ simp[hello_init_memory_def]
+    \\ simp[wordcount_init_memory_def]
     \\ rewrite_tac[GSYM WORD_ADD_ASSOC]
-    \\ `∀x:word32. get_byte (n2w n + x) = get_byte x`
-    by (
-      simp[Once ADD_COMM]
-      \\ `(n2w n : word32) = byte_align ((n2w n):word32)`
-      by ( fs[alignmentTheory.byte_aligned_def, alignmentTheory.byte_align_def, alignmentTheory.aligned_def] )
-      \\ pop_assum SUBST1_TAC
-      \\ simp[FUN_EQ_THM]
-      \\ rpt gen_tac
-      \\ match_mp_tac data_to_word_memoryProofTheory.get_byte_byte_align
-      \\ EVAL_TAC )
-    \\ simp[]
     \\ `∀(y:word32) x. get_byte (n2w (4 * x) + y) = get_byte y`
     by (
       rw[FUN_EQ_THM]
@@ -1257,23 +1055,6 @@ val hello_installed = Q.store_thm("hello_installed",
     \\ simp[]
     \\ pop_assum(qspec_then`0w`mp_tac) \\ simp[]
     \\ disch_then kall_tac
-    \\ `∀x:word32. byte_align (n2w n + x) = byte_align x + n2w n`
-    by (
-      `(n2w n : word32) = byte_align ((n2w n):word32)`
-      by ( fs[alignmentTheory.byte_aligned_def, alignmentTheory.byte_align_def, alignmentTheory.aligned_def] )
-      \\ fs[alignmentTheory.byte_aligned_def, alignmentTheory.byte_align_def]
-      \\ gen_tac
-      \\ once_rewrite_tac[WORD_ADD_COMM]
-      \\ DEP_REWRITE_TAC[align_add_aligned_gen]
-      \\ simp[] )
-    \\ rewrite_tac[GSYM WORD_ADD_ASSOC]
-    \\ simp[]
-    \\ rewrite_tac[GSYM WORD_ADD_ASSOC]
-    \\ qmatch_goalsub_abbrev_tac`(_:word32) + zz`
-    \\ `zz = 0w`
-    by ( simp[Abbr`zz`, word_add_n2w] )
-    \\ qpat_x_assum`Abbrev(zz = _)`kall_tac
-    \\ rw[]
     \\ `∀y x. byte_align (n2w (4 * x) + y) = n2w (4 * x) + byte_align y : word32`
     by (
       rw[]
@@ -1292,12 +1073,12 @@ val hello_installed = Q.store_thm("hello_installed",
     \\ simp[MULT_DIV]
     \\ qmatch_goalsub_abbrev_tac`get_byte _ mm`
     \\ pop_assum mp_tac
-    \\ rewrite_tac[hello_init_memory_words_def]
+    \\ rewrite_tac[wordcount_init_memory_words_def]
     \\ DEP_REWRITE_TAC[EL_APPEND2]
     \\ qmatch_goalsub_abbrev_tac`ll ≤ _`
     \\ pop_assum mp_tac
-    \\ simp[LENGTH_words_of_bytes_hello_startup_code,LENGTH_ag32_ffi_code,heap_size_def,
-            output_buffer_size_def,startup_code_size_def,LENGTH_hello_startup_code,
+    \\ simp[LENGTH_words_of_bytes_wordcount_startup_code,LENGTH_ag32_ffi_code,heap_size_def,
+            output_buffer_size_def,startup_code_size_def,LENGTH_wordcount_startup_code,
             LENGTH_ag32_ffi_jumps, ffi_names]
     \\ simp[LENGTH_words_of_bytes, bitstringTheory.length_pad_right, LENGTH_code,
             bytes_in_word_def, LENGTH_FLAT, MAP_MAP_o, o_DEF, ADD1, SUM_MAP_PLUS,
@@ -1310,7 +1091,14 @@ val hello_installed = Q.store_thm("hello_installed",
     \\ qpat_x_assum`Abbrev(cz = _)`kall_tac
     \\ rveq
     \\ rw[stdin_size_def, cline_size_def]
-    \\ simp[data_to_word_memoryProofTheory.word_of_bytes_def]
+    \\ simp[data_to_word_memoryProofTheory.word_of_bytes_def, Abbr`ll`]
+    \\ fs[LENGTH_data, LEFT_ADD_DISTRIB, Abbr`n`]
+    >- ( DEP_REWRITE_TAC[ADD_DIV_RWT] \\ simp[] )
+    \\ pop_assum mp_tac
+    \\ simp[]
+    \\ DEP_REWRITE_TAC[ADD_DIV_RWT] \\ simp[]
+    \\ once_rewrite_tac[MULT_COMM]
+    \\ simp[MULT_DIV] \\ rw[]
     \\ simp[wordSemTheory.get_byte_def, wordSemTheory.byte_index_def,
             wordSemTheory.set_byte_def, wordSemTheory.word_slice_alt_def]
     \\ blastLib.BBLAST_TAC)
@@ -1318,21 +1106,20 @@ val hello_installed = Q.store_thm("hello_installed",
   \\ rewrite_tac[ffi_names]
   \\ EVAL_TAC);
 
-val hello_machine_sem =
+val wordcount_machine_sem =
   compile_correct_applied
-  |> C MATCH_MP (UNDISCH hello_installed)
+  |> C MATCH_MP (UNDISCH wordcount_installed)
   |> DISCH_ALL
-  |> curry save_thm "hello_machine_sem";
+  |> curry save_thm "wordcount_machine_sem";
 
-val hello_halted = Q.store_thm("hello_halted",
+val wordcount_halted = Q.store_thm("wordcount_halted",
   `∀ms.
-    byte_aligned r0 ∧ w2n r0 + memory_size < dimword (:32) ∧
     SUM (MAP strlen cl) + LENGTH cl ≤ cline_size ∧
     LENGTH inp ≤ stdin_size ∧
-    (mc = hello_machine_config r0) ∧
+    (mc = wordcount_machine_config) ∧
     (ms.PC = mc.halt_pc) ∧
     (∀x. mc.halt_pc <=+ x ∧ x <+ mc.halt_pc + 16w ⇒
-         (mc.target.get_byte ms x = (hello_init_memory r0 (cl,inp)) x)) ⇒
+         (mc.target.get_byte ms x = (wordcount_init_memory (cl,inp)) x)) ⇒
     ∀k. ((FUNPOW Next k ms).io_events = ms.io_events) ∧
         ((FUNPOW Next k ms).PC = ms.PC) ∧
         ((FUNPOW Next k ms).MEM = ms.MEM) ∧
@@ -1348,11 +1135,7 @@ val hello_halted = Q.store_thm("hello_halted",
   \\ `aligned 2 pc`
   by (
     simp[Abbr`pc`]
-    \\ simp[hello_machine_config_def, ag32_machine_config_def]
-    \\ (alignmentTheory.aligned_add_sub_cor
-        |> SPEC_ALL |> UNDISCH |> CONJUNCT1 |> DISCH_ALL
-        |> irule)
-    \\ fs[alignmentTheory.byte_aligned_def]
+    \\ simp[wordcount_machine_config_def, ag32_machine_config_def]
     \\ simp[LENGTH_data, heap_size_def, lab_to_targetTheory.ffi_offset_def, ffi_names]
     \\ EVAL_TAC )
   \\ `pc = pc'`
@@ -1365,41 +1148,20 @@ val hello_halted = Q.store_thm("hello_halted",
   \\ pop_assum (SUBST_ALL_TAC o SYM)
   \\ fs[Abbr`pc`]
   \\ first_assum(qspec_then`ms.PC`mp_tac)
-  \\ impl_tac
-  >- (
-    simp[]
-    \\ Cases_on`r0`
-    \\ fs[word_add_n2w,word_ls_n2w,word_lo_n2w,memory_size_def]
-    \\ simp[hello_machine_config_halt_pc, word_add_n2w]
-    \\ fs[word_add_n2w,word_ls_n2w,word_lo_n2w,memory_size_def] )
+  \\ impl_tac >- simp[wordcount_machine_config_halt_pc]
   \\ first_assum(qspec_then`ms.PC + 1w`mp_tac)
-  \\ impl_tac
-  >- (
-    simp[]
-    \\ Cases_on`r0`
-    \\ simp[hello_machine_config_halt_pc]
-    \\ fs[word_add_n2w,word_ls_n2w,word_lo_n2w,memory_size_def] )
+  \\ impl_tac >- simp[wordcount_machine_config_halt_pc]
   \\ first_assum(qspec_then`ms.PC + 2w`mp_tac)
-  \\ impl_tac
-  >- (
-    simp[]
-    \\ Cases_on`r0`
-    \\ simp[hello_machine_config_halt_pc]
-    \\ fs[word_add_n2w,word_ls_n2w,word_lo_n2w,memory_size_def] )
+  \\ impl_tac >- simp[wordcount_machine_config_halt_pc]
   \\ first_x_assum(qspec_then`ms.PC + 3w`mp_tac)
-  \\ impl_tac
-  >- (
-    simp[]
-    \\ Cases_on`r0`
-    \\ simp[hello_machine_config_halt_pc]
-    \\ fs[word_add_n2w,word_ls_n2w,word_lo_n2w,memory_size_def] )
+  \\ impl_tac >- simp[wordcount_machine_config_halt_pc]
   \\ simp[]
-  \\ simp[EVAL``(hello_machine_config r0).target.get_byte``]
+  \\ simp[EVAL``(wordcount_machine_config).target.get_byte``]
   \\ rpt (disch_then SUBST_ALL_TAC)
-  \\ qmatch_goalsub_abbrev_tac`_ @@ hello_init_memory r0 _ pc`
-  \\ drule hello_init_memory_halt
+  \\ qmatch_goalsub_abbrev_tac`_ @@ wordcount_init_memory _ pc`
+  \\ mp_tac wordcount_init_memory_halt
   \\ impl_tac >- simp[]
-  \\ simp[]
+  \\ simp[get_mem_word_def]
   \\ disch_then kall_tac
   \\ simp[ag32_targetProofTheory.Decode_Encode]
   \\ simp[ag32Theory.Run_def, ag32Theory.dfn'Jump_def]
@@ -1407,27 +1169,26 @@ val hello_halted = Q.store_thm("hello_halted",
   \\ strip_tac
   \\ simp[Abbr`ms1`, APPLY_UPDATE_THM]);
 
-val hello_interference_implemented = Q.store_thm("hello_interference_implemented",
-  `Abbrev (r0 = n2w ZERO) ∧ byte_aligned r0 ∧ w2n r0 + memory_size < dimword (:32) ∧
-   SUM (MAP strlen cl) + LENGTH cl ≤ cline_size ∧
+val wordcount_interference_implemented = Q.store_thm("wordcount_interference_implemented",
+  `SUM (MAP strlen cl) + LENGTH cl ≤ cline_size ∧
    LENGTH inp ≤ stdin_size ∧
-   is_ag32_init_state (hello_init_memory r0 (cl,inp)) ms0 ∧
-   Abbrev(ms = FUNPOW Next (hello_startup_clock r0 ms0 inp cl) ms0)
+   is_ag32_init_state (wordcount_init_memory (cl,inp)) ms0 ∧
+   Abbrev(ms = FUNPOW Next (wordcount_startup_clock ms0 inp cl) ms0)
   ⇒
    interference_implemented
-    (hello_machine_config r0)
-    (ag32_ffi_rel r0)
-    (ag32_ffi_mem_domain r0) ms`,
+    (wordcount_machine_config)
+    (ag32_ffi_rel 0w)
+    (ag32_ffi_mem_domain 0w) ms`,
   rw[interference_implemented_def]
-  \\ simp[EVAL``(hello_machine_config r0).target.next``]
-  \\ simp[EVAL``(hello_machine_config r0).target.get_byte``]
-  \\ simp[EVAL``(hello_machine_config r0).target.get_pc``]
-  \\ simp[EVAL``(hello_machine_config r0).target.get_reg``]
-  \\ simp[EVAL``(hello_machine_config r0).ffi_entry_pcs``]
+  \\ simp[EVAL``(wordcount_machine_config).target.next``]
+  \\ simp[EVAL``(wordcount_machine_config).target.get_byte``]
+  \\ simp[EVAL``(wordcount_machine_config).target.get_pc``]
+  \\ simp[EVAL``(wordcount_machine_config).target.get_reg``]
+  \\ simp[EVAL``(wordcount_machine_config).ffi_entry_pcs``]
   \\ simp[ffi_names]
-  \\ simp[Once hello_machine_config_def, ag32_machine_config_def]
-  \\ simp[Once hello_machine_config_def, ag32_machine_config_def]
-  \\ simp[Once hello_machine_config_def, ag32_machine_config_def]
+  \\ simp[Once wordcount_machine_config_def, ag32_machine_config_def]
+  \\ simp[Once wordcount_machine_config_def, ag32_machine_config_def]
+  \\ simp[Once wordcount_machine_config_def, ag32_machine_config_def]
   \\ qx_gen_tac`k0`
   \\ strip_tac
   \\ conj_tac
@@ -1441,7 +1202,7 @@ val hello_interference_implemented = Q.store_thm("hello_interference_implemented
     \\ `(Next ms1).io_events = ms1.io_events` suffices_by rw[]
     \\ irule ag32_io_events_unchanged
     \\ simp[Abbr`ms1`]
-    \\ `aligned 2 pc` by rfs[ag32_targetTheory.ag32_target_def, ag32_targetTheory.ag32_ok_def, EVAL``(hello_machine_config r0).target.state_ok``]
+    \\ `aligned 2 pc` by rfs[ag32_targetTheory.ag32_target_def, ag32_targetTheory.ag32_ok_def, EVAL``(wordcount_machine_config).target.state_ok``]
     \\ qmatch_goalsub_abbrev_tac`m (pc' + _)`
     \\ `pc' = pc`
     by (
@@ -1452,8 +1213,8 @@ val hello_interference_implemented = Q.store_thm("hello_interference_implemented
     \\ qpat_x_assum`Abbrev(pc' = _)`kall_tac
     \\ pop_assum SUBST_ALL_TAC
     \\ fs[targetSemTheory.encoded_bytes_in_mem_def]
-    \\ fs[EVAL``(hello_machine_config r0).target.config.code_alignment``]
-    \\ fs[EVAL``(hello_machine_config r0).target.config.encode``]
+    \\ fs[EVAL``(wordcount_machine_config).target.config.code_alignment``]
+    \\ fs[EVAL``(wordcount_machine_config).target.config.encode``]
     \\ `4 ≤ LENGTH (DROP (4 * k) (ag32_enc i))` by (
       qspec_then`i`mp_tac(Q.GEN`istr`ag32_enc_lengths)
       \\ simp[]
@@ -1493,11 +1254,7 @@ val hello_interference_implemented = Q.store_thm("hello_interference_implemented
       \\ qmatch_asmsub_abbrev_tac`_.PC = pc`
       \\ `aligned 2 pc`
       by (
-        simp[Abbr`pc`, hello_machine_config_ccache_pc]
-        \\ (alignmentTheory.aligned_add_sub_cor
-            |> SPEC_ALL |> UNDISCH |> CONJUNCT1 |> DISCH_ALL
-            |> irule)
-        \\ fs[alignmentTheory.byte_aligned_def]
+        simp[Abbr`pc`, wordcount_machine_config_ccache_pc]
         \\ EVAL_TAC )
       \\ `pc = pc'`
       by (
@@ -1508,77 +1265,34 @@ val hello_interference_implemented = Q.store_thm("hello_interference_implemented
       \\ qpat_x_assum`Abbrev(pc' = _)` kall_tac
       \\ pop_assum (SUBST_ALL_TAC o SYM)
       \\ first_assum(qspec_then`pc`mp_tac)
-      \\ impl_tac
-      >- (
-        simp[Abbr`pc`]
-        \\ EVAL_TAC \\ simp[ffi_names, LENGTH_code, LENGTH_data]
-        \\ Cases_on`r0`
-        \\ fs[word_add_n2w,word_ls_n2w,word_lo_n2w,memory_size_def] )
+      \\ impl_tac >- ( simp[Abbr`pc`] \\ EVAL_TAC \\ simp[ffi_names, LENGTH_code, LENGTH_data])
       \\ first_assum(qspec_then`pc + 1w`mp_tac)
-      \\ impl_tac
-      >- (
-        simp[Abbr`pc`]
-        \\ EVAL_TAC \\ simp[ffi_names, LENGTH_code, LENGTH_data]
-        \\ Cases_on`r0`
-        \\ fs[word_add_n2w,word_ls_n2w,word_lo_n2w,memory_size_def] )
+      \\ impl_tac >- ( simp[Abbr`pc`] \\ EVAL_TAC \\ simp[ffi_names, LENGTH_code, LENGTH_data])
       \\ first_assum(qspec_then`pc + 2w`mp_tac)
-      \\ impl_tac
-      >- (
-        simp[Abbr`pc`]
-        \\ EVAL_TAC \\ simp[ffi_names, LENGTH_code, LENGTH_data]
-        \\ Cases_on`r0`
-        \\ fs[word_add_n2w,word_ls_n2w,word_lo_n2w,memory_size_def] )
+      \\ impl_tac >- ( simp[Abbr`pc`] \\ EVAL_TAC \\ simp[ffi_names, LENGTH_code, LENGTH_data])
       \\ first_assum(qspec_then`pc + 3w`mp_tac)
-      \\ impl_tac
-      >- (
-        simp[Abbr`pc`]
-        \\ EVAL_TAC \\ simp[ffi_names, LENGTH_code, LENGTH_data]
-        \\ Cases_on`r0`
-        \\ fs[word_add_n2w,word_ls_n2w,word_lo_n2w,memory_size_def] )
+      \\ impl_tac >- ( simp[Abbr`pc`] \\ EVAL_TAC \\ simp[ffi_names, LENGTH_code, LENGTH_data])
       \\ simp[]
       \\ ntac 4 (disch_then kall_tac)
-      \\ drule hello_startup_clock_def
+      \\ mp_tac wordcount_startup_clock_def
       \\ simp[]
       \\ disch_then drule
       \\ disch_then drule
       \\ disch_then drule
       \\ strip_tac
       \\ first_assum(qspec_then`pc`mp_tac)
-      \\ impl_tac
-      >- (
-        simp[Abbr`pc`]
-        \\ EVAL_TAC
-        \\ simp[ffi_names,LENGTH_code,LENGTH_data]
-        \\ Cases_on`r0`
-        \\ fs[word_add_n2w,word_ls_n2w,word_lo_n2w,memory_size_def] )
+      \\ impl_tac >- ( simp[Abbr`pc`] \\ EVAL_TAC \\ simp[ffi_names,LENGTH_code,LENGTH_data])
       \\ first_assum(qspec_then`pc + 1w`mp_tac)
-      \\ impl_tac
-      >- (
-        simp[Abbr`pc`]
-        \\ EVAL_TAC
-        \\ simp[ffi_names,LENGTH_code,LENGTH_data]
-        \\ Cases_on`r0`
-        \\ fs[word_add_n2w,word_ls_n2w,word_lo_n2w,memory_size_def] )
+      \\ impl_tac >- ( simp[Abbr`pc`] \\ EVAL_TAC \\ simp[ffi_names,LENGTH_code,LENGTH_data])
       \\ first_assum(qspec_then`pc + 2w`mp_tac)
-      \\ impl_tac
-      >- (
-        simp[Abbr`pc`]
-        \\ EVAL_TAC
-        \\ simp[ffi_names,LENGTH_code,LENGTH_data]
-        \\ Cases_on`r0`
-        \\ fs[word_add_n2w,word_ls_n2w,word_lo_n2w,memory_size_def] )
+      \\ impl_tac >- ( simp[Abbr`pc`] \\ EVAL_TAC \\ simp[ffi_names,LENGTH_code,LENGTH_data])
       \\ first_assum(qspec_then`pc + 3w`mp_tac)
-      \\ impl_tac
-      >- (
-        simp[Abbr`pc`]
-        \\ EVAL_TAC
-        \\ simp[ffi_names,LENGTH_code,LENGTH_data]
-        \\ Cases_on`r0`
-        \\ fs[word_add_n2w,word_ls_n2w,word_lo_n2w,memory_size_def] )
+      \\ impl_tac >- ( simp[Abbr`pc`] \\ EVAL_TAC \\ simp[ffi_names,LENGTH_code,LENGTH_data])
       \\ simp[]
       \\ ntac 4 (disch_then kall_tac)
       \\ fs[is_ag32_init_state_def]
-      \\ DEP_REWRITE_TAC[hello_init_memory_ccache]
+      \\ simp[GSYM get_mem_word_def]
+      \\ DEP_REWRITE_TAC[wordcount_init_memory_ccache]
       \\ conj_tac
       >- ( simp[Abbr`pc`,LENGTH_data] \\ EVAL_TAC )
       \\ simp[ag32_targetProofTheory.Decode_Encode]
@@ -1587,7 +1301,7 @@ val hello_interference_implemented = Q.store_thm("hello_interference_implemented
       \\ simp[ag32Theory.ALU_def]
       \\ simp[ag32Theory.ri2word_def]
       \\ rpt(AP_TERM_TAC ORELSE AP_THM_TAC)
-      \\ simp[Abbr`pc`, hello_machine_config_ccache_pc,ffi_names]
+      \\ simp[Abbr`pc`, wordcount_machine_config_ccache_pc,ffi_names]
       \\ EVAL_TAC)
     \\ pop_assum(SUBST_ALL_TAC o SYM)
     \\ conj_tac >- simp[ag32_ffi_rel_def,FUN_EQ_THM]
@@ -1596,7 +1310,7 @@ val hello_interference_implemented = Q.store_thm("hello_interference_implemented
   \\ strip_tac
   \\ fs[find_index_def] \\ rveq
   \\ simp[ffi_names]
-  \\ fs[EVAL``(hello_machine_config r0).ffi_names``, ffi_names]
+  \\ fs[EVAL``(wordcount_machine_config).ffi_names``, ffi_names]
   \\ fs[ffiTheory.call_FFI_def,CaseEq"oracle_result",CaseEq"bool"]
   \\ rveq \\ rfs[basis_ffiTheory.basis_ffi_def]
   \\ `ffi.oracle = basis_ffi_oracle` by fs[ag32_ffi_rel_def] \\ fs[]
@@ -1605,23 +1319,25 @@ val hello_interference_implemented = Q.store_thm("hello_interference_implemented
   \\ pairarg_tac \\ rw[CaseEq"option",CaseEq"ffi_result"]
   \\ qmatch_goalsub_abbrev_tac`_ = FUNPOW Next _ ms1`
   \\ drule (GEN_ALL ag32_ffi_interfer_write)
-  \\ fs[hello_machine_config_def]
+  \\ fs[wordcount_machine_config_def]
   \\ disch_then drule
-  \\ fs[GSYM hello_machine_config_def]
+  \\ fs[GSYM wordcount_machine_config_def]
   \\ simp[ffiTheory.call_FFI_def, Once basis_ffiTheory.basis_ffi_oracle_def]
   \\ simp[ffi_names, INDEX_OF_def, INDEX_FIND_def]
   \\ reverse impl_tac
   THEN1
    (strip_tac
     \\ asm_exists_tac
-    \\ simp[hello_machine_config_def,ag32_machine_config_def])
+    \\ simp[wordcount_machine_config_def,ag32_machine_config_def])
+  \\ conj_tac >- EVAL_TAC
+  \\ conj_tac >- EVAL_TAC
   \\ conj_tac
   >- (
     fs[targetSemTheory.read_ffi_bytearrays_def,
        targetSemTheory.read_ffi_bytearray_def,
-       EVAL``(hello_machine_config r0).target.get_reg``,
-       EVAL``(hello_machine_config r0).ptr2_reg``,
-       EVAL``(hello_machine_config r0).len2_reg``]
+       EVAL``(wordcount_machine_config).target.get_reg``,
+       EVAL``(wordcount_machine_config).ptr2_reg``,
+       EVAL``(wordcount_machine_config).len2_reg``]
     \\ drule (SIMP_RULE(srw_ss())[PULL_EXISTS, IS_SOME_EXISTS]read_bytearray_no_wrap)
     \\ simp[]
     \\ Cases_on`ms1.R 4w` \\ fs[]
@@ -1633,8 +1349,6 @@ val hello_interference_implemented = Q.store_thm("hello_interference_implemented
     \\ simp[ffi_names, LENGTH_code, LENGTH_data]
     \\ qpat_x_assum`_ = ms1.PC`(assume_tac o SYM)
     \\ simp[]
-    \\ `r0 = n2w 0` by metis_tac[ALT_ZERO]
-    \\ simp[]
     \\ Cases
     \\ simp[word_ls_n2w, word_lo_n2w] )
   \\ conj_tac >- EVAL_TAC
@@ -1643,15 +1357,14 @@ val hello_interference_implemented = Q.store_thm("hello_interference_implemented
   \\ conj_tac >- (
     rw[]
     \\ first_assum(mp_then Any mp_tac (GEN_ALL get_mem_word_get_byte))
-    \\ disch_then(first_assum o mp_then Any mp_tac)
     \\ disch_then(qspec_then`ffi_jumps_offset DIV 4`mp_tac)
     \\ simp[LEFT_ADD_DISTRIB]
     \\ mp_tac(EVAL``4 * (ffi_jumps_offset DIV 4) = ffi_jumps_offset``)
     \\ simp[] \\ disch_then kall_tac
     \\ disch_then match_mp_tac
     \\ qexists_tac`DROP (ffi_jumps_offset DIV 4 + LENGTH (ag32_ffi_jumps (THE config.ffi_names)))
-                        (hello_init_memory_words cl inp)`
-    \\ qexists_tac`TAKE (ffi_jumps_offset DIV 4) (hello_init_memory_words cl inp)`
+                        (wordcount_init_memory_words cl inp)`
+    \\ qexists_tac`TAKE (ffi_jumps_offset DIV 4) (wordcount_init_memory_words cl inp)`
     \\ simp[ffi_names]
     \\ reverse conj_tac
     >- (
@@ -1660,39 +1373,39 @@ val hello_interference_implemented = Q.store_thm("hello_interference_implemented
       >- (
         pop_assum mp_tac
         \\ EVAL_TAC
-        \\ Cases_on`r0` \\ fs[memory_size_def] )
+        \\ fs[])
       \\ rw[]
       \\ pop_assum mp_tac
       \\ simp[]
       \\ CONV_TAC(LAND_CONV EVAL)
-      \\ simp[LENGTH_hello_init_memory_words] )
+      \\ simp[LENGTH_wordcount_init_memory_words] )
     \\ simp[LENGTH_TAKE_EQ]
     \\ reverse IF_CASES_TAC
     >- (
       `F` suffices_by rw[]
       \\ pop_assum mp_tac
-      \\ simp[LENGTH_hello_init_memory_words]
+      \\ simp[LENGTH_wordcount_init_memory_words]
       \\ EVAL_TAC )
     \\ rw[]
     \\ qmatch_goalsub_abbrev_tac`EL _ mw`
-    \\ `mw = hello_init_memory_words cl inp`
+    \\ `mw = wordcount_init_memory_words cl inp`
     by (
       simp[Abbr`mw`]
       \\ match_mp_tac TAKE_DROP_SUBLIST
       \\ simp[]
       \\ reverse conj_tac
       >- (
-        simp[LENGTH_hello_init_memory_words]
+        simp[LENGTH_wordcount_init_memory_words]
         \\ EVAL_TAC )
       \\ simp[IS_PREFIX_APPEND]
-      \\ simp[hello_init_memory_words_def]
+      \\ simp[wordcount_init_memory_words_def]
       \\ simp[ffi_names]
       \\ qmatch_goalsub_abbrev_tac`l1 ++ ag32_ffi_jumps _ ++ _ ++ _`
       \\ `ffi_jumps_offset DIV 4 = LENGTH l1`
       by (
         simp[Abbr`l1`, LENGTH_ag32_ffi_code, heap_size_def,
-             output_buffer_size_def, LENGTH_hello_startup_code,
-             startup_code_size_def,LENGTH_words_of_bytes_hello_startup_code]
+             output_buffer_size_def, LENGTH_wordcount_startup_code,
+             startup_code_size_def,LENGTH_words_of_bytes_wordcount_startup_code]
         \\ CONV_TAC(LAND_CONV EVAL)
         \\ simp[LENGTH_words_of_bytes, bitstringTheory.length_pad_right, LENGTH_code,
                 bytes_in_word_def, LENGTH_FLAT, MAP_MAP_o, o_DEF, ADD1, SUM_MAP_PLUS,
@@ -1710,8 +1423,8 @@ val hello_interference_implemented = Q.store_thm("hello_interference_implemented
       \\ simp[])
     \\ qpat_x_assum`Abbrev(mw = _)`kall_tac
     \\ rw[]
-    \\ simp[GSYM(SIMP_RULE(srw_ss())[]hello_init_memory_def)]
-    \\ drule hello_startup_clock_def
+    \\ simp[GSYM(SIMP_RULE(srw_ss())[]wordcount_init_memory_def)]
+    \\ mp_tac wordcount_startup_clock_def
     \\ simp[]
     \\ rpt(disch_then drule)
     \\ rw[]
@@ -1720,17 +1433,17 @@ val hello_interference_implemented = Q.store_thm("hello_interference_implemented
     \\ `ms1.MEM x = ms.MEM x`
     by (
       first_x_assum irule
-      \\ simp[hello_machine_config_def, ag32_machine_config_def]
+      \\ simp[wordcount_machine_config_def, ag32_machine_config_def]
       \\ conj_tac
       >- (
         EVAL_TAC
         \\ fs[EVAL``ffi_jumps_offset``, EVAL``ag32_ffi_jumps [_]``]
-        \\ Cases_on`x` \\ Cases_on`r0` \\ fs[memory_size_def, word_add_n2w]
+        \\ Cases_on`x` \\ fs[ word_add_n2w]
         \\ fs[word_ls_n2w, word_lo_n2w] \\ rfs[] )
       \\ simp[ffi_names, LENGTH_code, LENGTH_data]
       \\ qpat_x_assum`_ = ms1.PC`(assume_tac o SYM)
       \\ EVAL_TAC \\ simp[]
-      \\ Cases_on`x` \\ Cases_on`r0` \\ fs[memory_size_def, word_add_n2w]
+      \\ Cases_on`x` \\ fs[word_add_n2w]
       \\ fs[word_ls_n2w, word_lo_n2w] \\ rfs[]
       \\ fs[EVAL``ffi_jumps_offset``, EVAL``ag32_ffi_jumps [_]``]
       \\ rfs[])
@@ -1738,43 +1451,43 @@ val hello_interference_implemented = Q.store_thm("hello_interference_implemented
     \\ first_x_assum irule
     \\ EVAL_TAC
     \\ fs[EVAL``ffi_jumps_offset``, EVAL``ag32_ffi_jumps [_]``]
-    \\ Cases_on`r0` \\ Cases_on`x` \\ Cases_on`ms0.PC` \\ fs[memory_size_def, word_add_n2w]
+    \\ Cases_on`x` \\ Cases_on`ms0.PC` \\ fs[word_add_n2w]
     \\ fs[word_ls_n2w, word_lo_n2w] \\ rfs[])
   \\ rw[]
-  \\ first_assum(mp_then Any mp_tac (GEN_ALL get_mem_word_get_byte))
   \\ qmatch_goalsub_abbrev_tac`4 * k + off`
-  \\ disch_then(qspecl_then[`off DIV 4`,`ms1.MEM`,`MAP Encode ag32_ffi_write_code`]mp_tac)
+  \\ qspecl_then[`off DIV 4`,`ms1.MEM`,`MAP Encode ag32_ffi_write_code`]mp_tac
+      (GEN_ALL get_mem_word_get_byte)
   \\ simp[EL_MAP,LEFT_ADD_DISTRIB]
   \\ `4 * (off DIV 4) = off` by (simp[Abbr`off`] \\ EVAL_TAC)
   \\ simp[]
   \\ disch_then match_mp_tac
   \\ pop_assum kall_tac
-  \\ qexists_tac`DROP (off DIV 4 + LENGTH ag32_ffi_write_code) (hello_init_memory_words cl inp)`
-  \\ qexists_tac`TAKE (off DIV 4) (hello_init_memory_words cl inp)`
+  \\ qexists_tac`DROP (off DIV 4 + LENGTH ag32_ffi_write_code) (wordcount_init_memory_words cl inp)`
+  \\ qexists_tac`TAKE (off DIV 4) (wordcount_init_memory_words cl inp)`
   \\ reverse conj_tac
   >- (
-    simp[LENGTH_TAKE_EQ, LENGTH_hello_init_memory_words]
+    simp[LENGTH_TAKE_EQ, LENGTH_wordcount_init_memory_words]
     \\ simp[Abbr`off`]
     \\ pop_assum mp_tac
     \\ EVAL_TAC
     \\ fs[memory_size_def] )
-  \\ simp[LENGTH_TAKE_EQ, LENGTH_hello_init_memory_words]
+  \\ simp[LENGTH_TAKE_EQ, LENGTH_wordcount_init_memory_words]
   \\ pop_assum mp_tac
   \\ CONV_TAC(LAND_CONV EVAL)
   \\ strip_tac \\ simp[Abbr`off`]
   \\ rw[]
   \\ qmatch_goalsub_abbrev_tac`EL _ mw`
-  \\ `mw = hello_init_memory_words cl inp`
+  \\ `mw = wordcount_init_memory_words cl inp`
   by (
     simp[Abbr`mw`]
     \\ match_mp_tac TAKE_DROP_SUBLIST
     \\ simp[]
     \\ reverse conj_tac
     >- (
-      simp[LENGTH_hello_init_memory_words]
+      simp[LENGTH_wordcount_init_memory_words]
       \\ EVAL_TAC )
     \\ simp[IS_PREFIX_APPEND]
-    \\ simp[hello_init_memory_words_def]
+    \\ simp[wordcount_init_memory_words_def]
     \\ simp[ffi_names]
     \\ simp[ag32_ffi_code_def]
     \\ rewrite_tac[GSYM APPEND_ASSOC]
@@ -1785,8 +1498,8 @@ val hello_interference_implemented = Q.store_thm("hello_interference_implemented
     \\ `n = LENGTH l1`
     by (
       simp[Abbr`n`, Abbr`l1`, LENGTH_ag32_ffi_code, heap_size_def,
-           output_buffer_size_def, LENGTH_hello_startup_code,
-           startup_code_size_def,LENGTH_words_of_bytes_hello_startup_code]
+           output_buffer_size_def, LENGTH_wordcount_startup_code,
+           startup_code_size_def,LENGTH_words_of_bytes_wordcount_startup_code]
       \\ CONV_TAC(PATH_CONV"rrr"EVAL)
       \\ simp[LENGTH_words_of_bytes, bitstringTheory.length_pad_right, LENGTH_code,
               bytes_in_word_def, LENGTH_FLAT, MAP_MAP_o, o_DEF, ADD1, SUM_MAP_PLUS,
@@ -1804,8 +1517,8 @@ val hello_interference_implemented = Q.store_thm("hello_interference_implemented
     \\ simp[])
   \\ qpat_x_assum`Abbrev(mw = _)`kall_tac
   \\ rw[]
-  \\ simp[GSYM(SIMP_RULE(srw_ss())[]hello_init_memory_def)]
-  \\ drule hello_startup_clock_def
+  \\ simp[GSYM(SIMP_RULE(srw_ss())[]wordcount_init_memory_def)]
+  \\ mp_tac wordcount_startup_clock_def
   \\ simp[]
   \\ rpt(disch_then drule)
   \\ rw[]
@@ -1814,17 +1527,17 @@ val hello_interference_implemented = Q.store_thm("hello_interference_implemented
   \\ `ms1.MEM x = ms.MEM x`
   by (
     first_x_assum irule
-    \\ simp[hello_machine_config_def, ag32_machine_config_def]
+    \\ simp[wordcount_machine_config_def, ag32_machine_config_def]
     \\ conj_tac
     >- (
       EVAL_TAC
       \\ fs[EVAL``LENGTH ag32_ffi_write_code``]
-      \\ Cases_on`x` \\ Cases_on`r0` \\ fs[memory_size_def, word_add_n2w]
+      \\ Cases_on`x` \\ fs[word_add_n2w]
       \\ fs[word_ls_n2w, word_lo_n2w] \\ rfs[] )
     \\ simp[ffi_names, LENGTH_code, LENGTH_data]
     \\ qpat_x_assum`_ = ms1.PC`(assume_tac o SYM)
     \\ EVAL_TAC \\ simp[]
-    \\ Cases_on`x` \\ Cases_on`r0` \\ fs[memory_size_def, word_add_n2w]
+    \\ Cases_on`x` \\ fs[word_add_n2w]
     \\ fs[word_ls_n2w, word_lo_n2w] \\ rfs[]
     \\ fs[EVAL``LENGTH ag32_ffi_write_code``]
     \\ rfs[])
@@ -1832,15 +1545,15 @@ val hello_interference_implemented = Q.store_thm("hello_interference_implemented
   \\ first_x_assum irule
   \\ EVAL_TAC
   \\ fs[EVAL``LENGTH ag32_ffi_write_code``]
-  \\ Cases_on`r0` \\ Cases_on`x` \\ Cases_on`ms0.PC` \\ fs[memory_size_def, word_add_n2w]
+  \\ Cases_on`x` \\ Cases_on`ms0.PC` \\ fs[word_add_n2w]
   \\ fs[word_ls_n2w, word_lo_n2w] \\ rfs[]);
 
-val hello_extract_writes_stdout = Q.store_thm("hello_extract_writes_stdout",
+val wordcount_extract_writes_stdout = Q.store_thm("wordcount_extract_writes_stdout",
   `wfcl cl ∧ 2 ≤ maxFD ⇒
-   (extract_writes 1 (MAP get_output_io_event (hello_io_events cl (stdin_fs inp))) =
-    "Hello World!\n")`,
+   (extract_writes 1 (MAP get_output_io_event (wordcount_io_events cl (stdin_fs inp))) =
+    "wordcount World!\n")`,
   strip_tac
-  \\ drule(GEN_ALL(DISCH_ALL hello_output))
+  \\ drule(GEN_ALL(DISCH_ALL wordcount_output))
   \\ disch_then(qspec_then`stdin_fs inp`mp_tac)
   \\ simp[wfFS_stdin_fs, STD_streams_stdin_fs]
   \\ simp[TextIOProofTheory.add_stdo_def]
@@ -1870,25 +1583,23 @@ val hello_extract_writes_stdout = Q.store_thm("hello_extract_writes_stdout",
   >- rw[]
   >- rw[]);
 
-val hello_ag32_next = Q.store_thm("hello_ag32_next",
-  `Abbrev(r0 = n2w ZERO) ∧ byte_aligned r0 ∧ w2n r0 + memory_size < dimword (:32) ∧
-   SUM (MAP strlen cl) + LENGTH cl ≤ cline_size ∧ wfcl cl ∧
+val wordcount_ag32_next = Q.store_thm("wordcount_ag32_next",
+  `SUM (MAP strlen cl) + LENGTH cl ≤ cline_size ∧ wfcl cl ∧
    LENGTH inp ≤ stdin_size ∧ 2 ≤ maxFD ∧
-   is_ag32_init_state (hello_init_memory r0 (cl,inp)) ms0
+   is_ag32_init_state (wordcount_init_memory (cl,inp)) ms0
   ⇒
    ∃k1. ∀k. k1 ≤ k ⇒
      let ms = FUNPOW Next k ms0 in
-     let outs = MAP (get_ag32_io_event r0) ms.io_events in
-       (ms.PC = (hello_machine_config r0).halt_pc) ∧
-       outs ≼ MAP get_output_io_event (hello_io_events cl (stdin_fs inp)) ∧
-       ((ms.R (n2w (hello_machine_config r0).ptr_reg) = 0w) ⇒
-        (outs = MAP get_output_io_event (hello_io_events cl (stdin_fs inp))))`,
+     let outs = MAP (get_ag32_io_event 0w) ms.io_events in
+       (ms.PC = (wordcount_machine_config).halt_pc) ∧
+       outs ≼ MAP get_output_io_event (wordcount_io_events cl (stdin_fs inp)) ∧
+       ((ms.R (n2w (wordcount_machine_config).ptr_reg) = 0w) ⇒
+        (outs = MAP get_output_io_event (wordcount_io_events cl (stdin_fs inp))))`,
   rw[]
-  \\ drule (GEN_ALL hello_machine_sem)
+  \\ mp_tac (GEN_ALL wordcount_machine_sem)
   \\ disch_then(first_assum o mp_then Any mp_tac) \\ fs[]
   \\ disch_then(qspec_then`stdin_fs inp`mp_tac)
   \\ simp[wfFS_stdin_fs, STD_streams_stdin_fs]
-  \\ impl_tac >- rw[markerTheory.Abbrev_def]
   \\ strip_tac
   \\ fs[extend_with_resource_limit_def]
   \\ qmatch_asmsub_abbrev_tac`machine_sem mc st ms`
@@ -1898,7 +1609,7 @@ val hello_ag32_next = Q.store_thm("hello_ag32_next",
   \\ disch_then(assume_tac o ONCE_REWRITE_RULE[GSYM markerTheory.Abbrev_def])
   \\ `∃x y. b = Terminate x y` by fs[markerTheory.Abbrev_def] \\ rveq
   \\ first_x_assum(mp_then Any mp_tac (GEN_ALL machine_sem_Terminate_FUNPOW_next))
-  \\ drule hello_interference_implemented
+  \\ mp_tac wordcount_interference_implemented
   \\ impl_tac >- ( fs[] \\ fs[markerTheory.Abbrev_def] )
   \\ strip_tac \\ rfs[]
   \\ disch_then drule
@@ -1908,74 +1619,72 @@ val hello_ag32_next = Q.store_thm("hello_ag32_next",
     >- (
       EVAL_TAC
       \\ simp[Abbr`ms`]
-      \\ drule hello_startup_clock_def
+      \\ mp_tac wordcount_startup_clock_def
       \\ simp[]
       \\ rpt(disch_then drule)
       \\ fs[is_ag32_init_state_def])
     \\ simp[basis_ffiTheory.basis_ffi_def]
     \\ simp[ag32_fs_ok_stdin_fs])
   \\ strip_tac
-  \\ drule (GEN_ALL hello_halted)
+  \\ mp_tac (GEN_ALL wordcount_halted)
   \\ simp[]
   \\ disch_then drule
   \\ disch_then drule
   \\ disch_then(qspec_then`FUNPOW Next k ms`mp_tac)
   \\ strip_tac
-  \\ qexists_tac`k + hello_startup_clock r0 ms0 inp cl`
+  \\ qexists_tac`k + wordcount_startup_clock ms0 inp cl`
   \\ qx_gen_tac`k2` \\ strip_tac
-  \\ first_x_assum(qspec_then`k2-k-(hello_startup_clock r0 ms0 inp cl)`mp_tac)
+  \\ first_x_assum(qspec_then`k2-k-(wordcount_startup_clock ms0 inp cl)`mp_tac)
   \\ impl_tac
   >- (
     conj_tac
     >- (
       fs[Abbr`mc`]
-      \\ fs[EVAL``(hello_machine_config r0).target.get_pc``]
+      \\ fs[EVAL``(wordcount_machine_config).target.get_pc``]
       \\ fs[Abbr`ms`, FUNPOW_ADD]
-      \\ fs[EVAL``(hello_machine_config r0).target.next``]
+      \\ fs[EVAL``(wordcount_machine_config).target.next``]
       \\ first_x_assum irule
       \\ fs[markerTheory.Abbrev_def] )
     \\ fs[Abbr`mc`]
-    \\ fs[EVAL``(hello_machine_config r0).target.next``]
+    \\ fs[EVAL``(wordcount_machine_config).target.next``]
     \\ fs[Abbr`ms`, FUNPOW_ADD]
-    \\ drule hello_startup_clock_def
+    \\ mp_tac wordcount_startup_clock_def
     \\ disch_then(qspec_then`ms0`mp_tac)
     \\ disch_then(first_assum o mp_then Any mp_tac)
     \\ impl_tac >- fs[]
     \\ strip_tac
-    \\ fs[EVAL``(hello_machine_config r0).target.get_byte``]
+    \\ fs[EVAL``(wordcount_machine_config).target.get_byte``]
     \\ fs[ag32_targetTheory.is_ag32_init_state_def] \\ rfs[]
     \\ rw[]
     \\ qmatch_goalsub_rename_tac`_ = _ a`
-    \\ `a ∉ ag32_startup_addresses r0`
+    \\ `a ∉ ag32_startup_addresses 0w`
     by (
       EVAL_TAC
       \\ ntac 2 (pop_assum mp_tac)
       \\ EVAL_TAC
       \\ simp[ffi_names]
-      \\ Cases_on`r0` \\ Cases_on`a` \\ Cases_on`ms0.PC`
+      \\ Cases_on`a` \\ Cases_on`ms0.PC`
       \\ simp[word_add_n2w]
-      \\ simp[word_ls_n2w, word_lo_n2w]
-      \\ fs[memory_size_def] )
+      \\ simp[word_ls_n2w, word_lo_n2w])
     \\ first_x_assum drule
     \\ disch_then(assume_tac o SYM) \\ simp[]
     \\ first_x_assum irule
-    \\ Cases_on`r0` \\ Cases_on`a`
-    \\ fs[word_add_n2w, hello_machine_config_halt_pc]
-    \\ simp[hello_machine_config_def, ag32_machine_config_def, ffi_names, ag32_prog_addresses_def, LENGTH_code, LENGTH_data]
+    \\ Cases_on`a`
+    \\ fs[word_add_n2w, wordcount_machine_config_halt_pc]
+    \\ simp[wordcount_machine_config_def, ag32_machine_config_def, ffi_names, ag32_prog_addresses_def, LENGTH_code, LENGTH_data]
     \\ EVAL_TAC
     \\ fs[word_lo_n2w, word_ls_n2w, memory_size_def] \\ rfs[])
   \\ fs[GSYM FUNPOW_ADD, Abbr`ms`]
   \\ strip_tac
-  \\ fs[EVAL``(hello_machine_config r0).target.next``,Abbr`mc`,FUNPOW_ADD]
-  \\ fs[EVAL``(hello_machine_config r0).target.get_reg``]
-  \\ fs[EVAL``(hello_machine_config r0).target.get_pc``]
-  \\ fs[EVAL``(hello_machine_config r0).ptr_reg``]
+  \\ fs[EVAL``(wordcount_machine_config).target.next``,Abbr`mc`,FUNPOW_ADD]
+  \\ fs[EVAL``(wordcount_machine_config).target.get_reg``]
+  \\ fs[EVAL``(wordcount_machine_config).target.get_pc``]
+  \\ fs[EVAL``(wordcount_machine_config).ptr_reg``]
   \\ fs[ag32_ffi_rel_def]
   \\ conj_tac
   >- ( fs[IS_PREFIX_APPEND] \\ fs[markerTheory.Abbrev_def] )
   \\ strip_tac \\ fs[]
   \\ Cases_on`x` \\ fs[]
   \\ fs[markerTheory.Abbrev_def]);
-*)
 
 val _ = export_theory();
